store/db.v
@@ -39,14 +39,13 @@ Proof. solve_inG. Qed.
 
 Module DB.
 
-Definition N := nroot.@"db".
-
 Section DB.
 
 Implicit Types o : operationO.
 Implicit Types os : list operationO.
 Implicit Types db : gmap term term.
 Implicit Types γ : gname.
+Implicit Types N : namespace.
 Implicit Types n : nat.
 Implicit Types b : bool.
 Implicit Types T : coGset term.
@@ -66,26 +65,26 @@ Definition to_db os : gmap term term :=
 
 Context `{!cryptisGS Σ, !heapGS Σ, !dbGS Σ}.
 
-Definition hist_auth γ os : iProp Σ :=
+Definition hist_auth γ N os : iProp Σ :=
   nown γ (N.@"hist")
          (● to_max_prefix_list os ⋅ ◯ to_max_prefix_list os).
 
-Definition hist_frag γ os : iProp Σ :=
+Definition hist_frag γ N os : iProp Σ :=
   nown γ (N.@"hist")
          (◯ to_max_prefix_list os).
 
-Local Instance persistent_hist_frag γ os : Persistent (hist_frag γ os).
+Local Instance persistent_hist_frag γ N os : Persistent (hist_frag γ N os).
 Proof. apply _. Qed.
 
-Lemma hist_auth_frag γ os :
-  hist_auth γ os -∗
-  hist_frag γ os.
+Lemma hist_auth_frag γ N os :
+  hist_auth γ N os -∗
+  hist_frag γ N os.
 Proof. by iIntros "[_ Hown]". Qed.
 
-Lemma hist_frag_agree γ os1 os2 :
+Lemma hist_frag_agree γ N os1 os2 :
   length os1 = length os2 →
-  hist_frag γ os1 -∗
-  hist_frag γ os2 -∗
+  hist_frag γ N os1 -∗
+  hist_frag γ N os2 -∗
   ⌜os2 = os1⌝.
 Proof.
 move=> lengthE.
@@ -100,20 +99,20 @@ case: valid => - [[|o os] osE].
 - rewrite osE app_length /= in lengthE; lia.
 Qed.
 
-Lemma hist_frag_prefix_of os1 os2 γ :
+Lemma hist_frag_prefix_of os1 os2 γ N :
   os1 `prefix_of` os2 →
-  hist_frag γ os2 -∗
-  hist_frag γ os1.
+  hist_frag γ N os2 -∗
+  hist_frag γ N os1.
 Proof.
 iIntros "%os1_os2 #hist_frag". rewrite /hist_frag.
 iApply nown_mono; last by eauto.
 apply: auth_frag_mono. exact/to_max_prefix_list_included_L.
 Qed.
 
-Lemma hist_update γ os o :
-  hist_auth γ os ==∗
-  hist_auth γ (os ++ [o]) ∗
-  hist_frag γ (os ++ [o]).
+Lemma hist_update γ N os o :
+  hist_auth γ N os ==∗
+  hist_auth γ N (os ++ [o]) ∗
+  hist_frag γ N (os ++ [o]).
 Proof.
 iIntros "auth".
 iMod (nown_update with "auth") as "auth".
@@ -182,25 +181,25 @@ apply: option_local_update.
 by apply: exclusive_local_update.
 Qed.
 
-Definition state_auth γ db : iProp Σ :=
+Definition state_auth γ N db : iProp Σ :=
   nown γ (N.@"state") (db_state db).
 
-Definition mapsto γ t1 t2 : iProp Σ :=
+Definition mapsto γ N t1 t2 : iProp Σ :=
   nown γ (N.@"state") (db_singleton t1 t2).
 
-Definition free_at γ T : iProp Σ :=
+Definition free_at γ N T : iProp Σ :=
   nown γ (N.@"state") (db_free T).
 
-Lemma free_at_diff γ T1 T2 :
+Lemma free_at_diff γ N T1 T2 :
   T1 ⊆ T2 →
-  free_at γ T2 ⊣⊢ free_at γ T1 ∗ free_at γ (T2 ∖ T1).
+  free_at γ N T2 ⊣⊢ free_at γ N T1 ∗ free_at γ N (T2 ∖ T1).
 Proof.
 move=> sub. by rewrite /free_at db_free_diff // nown_op.
 Qed.
 
-Lemma state_auth_mapsto γ db t1 t2 :
-  state_auth γ db -∗
-  mapsto γ t1 t2 -∗
+Lemma state_auth_mapsto γ N db t1 t2 :
+  state_auth γ N db -∗
+  mapsto γ N t1 t2 -∗
   ⌜db !! t1 = Some t2⌝.
 Proof.
 iIntros "Hauth Hfrag".
@@ -212,11 +211,11 @@ case => incl _.
 by move/Excl_included/leibniz_equiv_iff: incl => <-.
 Qed.
 
-Lemma state_auth_update t2' γ db t1 t2 :
-  state_auth γ db -∗
-  mapsto γ t1 t2 ==∗
-  state_auth γ (<[t1 := t2']>db) ∗
-  mapsto γ t1 t2'.
+Lemma state_auth_update t2' γ N db t1 t2 :
+  state_auth γ N db -∗
+  mapsto γ N t1 t2 ==∗
+  state_auth γ N (<[t1 := t2']>db) ∗
+  mapsto γ N t1 t2'.
 Proof.
 iIntros "Hauth Hfrag".
 iMod (nown_update_2 with "Hauth Hfrag") as "own".
@@ -225,11 +224,11 @@ iDestruct "own" as "[Hauth Hfrag]".
 iModIntro. iSplitL "Hauth" => //.
 Qed.
 
-Lemma state_auth_create t1 t2 γ db :
-  state_auth γ db -∗
-  free_at γ {[t1]} ==∗
-  state_auth γ (op_app db (Create t1 t2)) ∗
-  mapsto γ t1 t2.
+Lemma state_auth_create t1 t2 γ N db :
+  state_auth γ N db -∗
+  free_at γ N {[t1]} ==∗
+  state_auth γ N (op_app db (Create t1 t2)) ∗
+  mapsto γ N t1 t2.
 Proof.
 iIntros "Hauth Hfree". rewrite /=.
 iAssert (⌜db !! t1 = None⌝)%I as "#->".
@@ -243,31 +242,31 @@ iMod (nown_update_2 _ _ (a' := (_ ⋅ _)) with "Hauth Hfree") as "[Hauth Hfrag]"
 iModIntro. iSplitL "Hauth" => //.
 Qed.
 
-Definition client_view γ n : iProp Σ :=
+Definition client_view γ N n : iProp Σ :=
   ∃ os,
     ⌜n = length os⌝ ∗
-    hist_auth γ os ∗
-    state_auth γ (to_db os).
+    hist_auth γ N os ∗
+    state_auth γ N (to_db os).
 
-Definition update_at γ n t1 t2 : iProp Σ :=
+Definition update_at γ N n t1 t2 : iProp Σ :=
   ∃ os, ⌜n = length os⌝ ∗
-        hist_frag γ (os ++ [Update t1 t2]).
+        hist_frag γ N (os ++ [Update t1 t2]).
 
-Definition create_at γ n t1 t2 : iProp Σ :=
+Definition create_at γ N n t1 t2 : iProp Σ :=
   ∃ os, ⌜n = length os⌝ ∗
-        hist_frag γ (os ++ [Create t1 t2]).
+        hist_frag γ N (os ++ [Create t1 t2]).
 
-Definition server_view γ n db : iProp Σ :=
+Definition server_view γ N n db : iProp Σ :=
   ∃ os, ⌜n = length os⌝ ∗
         ⌜db = to_db os⌝ ∗
-        hist_frag γ os.
+        hist_frag γ N os.
 
-Lemma alloc γ E :
+Lemma alloc γ N E :
   ↑N ⊆ E →
   gmeta_token γ E ==∗
-  client_view γ 0 ∗
-  free_at γ ⊤ ∗
-  server_view γ 0 ∅ ∗
+  client_view γ N 0 ∗
+  free_at γ N ⊤ ∗
+  server_view γ N 0 ∅ ∗
   gmeta_token γ (E ∖ ↑N).
 Proof.
 iIntros "%sub token".
@@ -283,7 +282,7 @@ iMod (nown_alloc (N.@"state") (db_state ∅ ⋅ db_free ⊤) with "token")
   rewrite -> decide_True; try set_solver.
   rewrite auth_both_valid_discrete Excl_included leibniz_equiv_iff.
   by split. }
-iAssert (hist_frag γ []) as "#frag".
+iAssert (hist_frag γ N []) as "#frag".
 { by iDestruct "hist" as "[??]". }
 iModIntro. iSplitR "free token".
 { iExists []. iSplit; eauto. iSplitL "hist" => //. }
@@ -293,15 +292,15 @@ iSplitR.
 iApply (gmeta_token_drop with "token"). solve_ndisj.
 Qed.
 
-Lemma update_client t2' γ n t1 t2 :
-  client_view γ n -∗
-  mapsto γ t1 t2 ==∗
-  client_view γ (S n) ∗
-  update_at γ n t1 t2' ∗
-  mapsto γ t1 t2'.
+Lemma update_client t2' γ N n t1 t2 :
+  client_view γ N n -∗
+  mapsto γ N t1 t2 ==∗
+  client_view γ N (S n) ∗
+  update_at γ N n t1 t2' ∗
+  mapsto γ N t1 t2'.
 Proof.
 iIntros "(%os & -> & own_os & own_db) own_frag".
-iMod (hist_update _ os (Update t1 t2') with "own_os") as "[auth_os #frag_os]".
+iMod (hist_update _ _ os (Update t1 t2') with "own_os") as "[auth_os #frag_os]".
 iMod (state_auth_update t2' with "own_db own_frag") as "[Hstate Hmapsto]".
 iModIntro. iSplitL "auth_os Hstate".
 { iExists (os ++ [Update t1 t2']).
@@ -311,13 +310,13 @@ iFrame.
 { iExists _; eauto. }
 Qed.
 
-Lemma update_server γ n db t1 t2 :
-  server_view γ n db -∗
-  update_at γ n t1 t2 -∗
-  server_view γ (S n) (<[t1 := t2]>db).
+Lemma update_server γ N n db t1 t2 :
+  server_view γ N n db -∗
+  update_at γ N n t1 t2 -∗
+  server_view γ N (S n) (<[t1 := t2]>db).
 Proof.
 iIntros "(%os & -> & -> & #frag) (%os' & %lengthE & #frag')".
-iPoseProof (hist_frag_agree _ lengthE with "frag []") as "->".
+iPoseProof (hist_frag_agree _ _ lengthE with "frag []") as "->".
 { iApply (hist_frag_prefix_of with "frag'").
   by exists [Update t1 t2]. }
 iExists (os ++ [Update t1 t2]). rewrite app_length Nat.add_comm /=.
@@ -325,15 +324,15 @@ do 2!iSplit => //.
 by rewrite /to_db foldl_app.
 Qed.
 
-Lemma create_client t1 t2 γ n :
-  client_view γ n -∗
-  free_at γ {[t1]} ==∗
-  create_at γ n t1 t2 ∗
-  client_view γ (S n) ∗
-  mapsto γ t1 t2.
+Lemma create_client t1 t2 γ N n :
+  client_view γ N n -∗
+  free_at γ N {[t1]} ==∗
+  create_at γ N n t1 t2 ∗
+  client_view γ N (S n) ∗
+  mapsto γ N t1 t2.
 Proof.
 iIntros "(%os & -> & hist & state) Hfree".
-iMod (hist_update _ _ (Create t1 t2) with "hist") as "[hist_auth #hist_frag]".
+iMod (hist_update _ _ _ (Create t1 t2) with "hist") as "[hist_auth #hist_frag]".
 iMod (state_auth_create t1 t2 with "state Hfree") as "[state mapsto]".
 have ->: op_app (to_db os) (Create t1 t2) = to_db (os ++ [Create t1 t2]).
 { by rewrite /to_db foldl_app. }
@@ -341,14 +340,14 @@ iModIntro. iFrame. iSplitR; first by iExists os; eauto.
 iExists _. iFrame. by rewrite app_length Nat.add_comm.
 Qed.
 
-Lemma create_server γ n db t1 t2 :
+Lemma create_server γ N n db t1 t2 :
   db !! t1 = None →
-  server_view γ n db -∗
-  create_at γ n t1 t2 -∗
-  server_view γ (S n) (<[t1 := t2]>db).
+  server_view γ N n db -∗
+  create_at γ N n t1 t2 -∗
+  server_view γ N (S n) (<[t1 := t2]>db).
 Proof.
 iIntros "%db_t1 (%os & -> & -> & #frag) (%os' & %lengthE & #frag')".
-iAssert (hist_frag γ os') as "#frag''".
+iAssert (hist_frag γ N os') as "#frag''".
 { iApply (hist_frag_prefix_of with "frag'").
   by exists [Create t1 t2]. }
 iPoseProof (hist_frag_agree with "frag frag''") as "->" => //.
@@ -356,15 +355,15 @@ iExists (os ++ [Create t1 t2]). rewrite app_length Nat.add_comm.
 do 2!iSplit => //. iPureIntro. by rewrite /to_db foldl_app /= db_t1.
 Qed.
 
-Definition stored_at γ n t1 t2 : iProp Σ :=
+Definition stored_at γ N n t1 t2 : iProp Σ :=
   ∃ os, ⌜n = length os⌝ ∗
-        hist_frag γ os ∗
+        hist_frag γ N os ∗
         ⌜to_db os !! t1 = Some t2⌝.
 
-Lemma load_client γ n t1 t2 t2' :
-  client_view γ n -∗
-  mapsto γ t1 t2 -∗
-  stored_at γ n t1 t2' -∗
+Lemma load_client γ N n t1 t2 t2' :
+  client_view γ N n -∗
+  mapsto γ N t1 t2 -∗
+  stored_at γ N n t1 t2' -∗
   ⌜t2' = t2⌝.
 Proof.
 iIntros "(%os & -> & hist & state) t1_t2 (%os' & %lengthE & #Hfrag & %os_t1)".
@@ -374,13 +373,41 @@ iPoseProof (state_auth_mapsto with "state t1_t2") as "%os_t1'".
 iPureIntro. rewrite os_t1 in os_t1'. by case: os_t1' => ->.
 Qed.
 
-Lemma load_server γ n db t1 t2 :
+Lemma load_server γ N n db t1 t2 :
   db !! t1 = Some t2 →
-  server_view γ n db -∗
-  stored_at γ n t1 t2.
+  server_view γ N n db -∗
+  stored_at γ N n t1 t2.
 Proof.
 iIntros "%db_t1 (%os & -> & -> & view)".
 iExists os; eauto.
+Qed.
+
+Lemma client_view_server_view γ N n :
+  client_view γ N n -∗ ∃ db,
+  server_view γ N n db.
+Proof.
+iIntros "(%os & %e_n & hist_auth & _)".
+iPoseProof (DB.hist_auth_frag with "hist_auth") as "#hist_frag".
+iExists _, os. do !iSplit => //.
+Qed.
+
+Lemma server_view_to_0 γ N n db :
+  server_view γ N n db -∗
+  server_view γ N 0 ∅.
+Proof.
+iIntros "(%os & %e_n & %e_db & hist_frag)".
+iExists [].
+do !iSplit => //.
+iApply (DB.hist_frag_prefix_of with "hist_frag").
+by exists os.
+Qed.
+
+Lemma server_view_0 γ N db :
+  server_view γ N 0 db -∗
+  ⌜db = ∅⌝.
+Proof.
+iIntros "(%os & %e_os & -> & #hist_frag)".
+case: os => // in e_os *.
 Qed.
 
 End DB.
