store/shared.v
@@ -3,8 +3,12 @@ From mathcomp Require Import ssreflect.
 From stdpp Require Import namespaces coGset.
 From iris.algebra Require Import agree auth csum gset gmap excl frac.
 From iris.algebra Require Import max_prefix_list.
+From iris.algebra.lib Require Import dfrac_agree.
+From iris.base_logic.lib Require Import invariants.
 From iris.heap_lang Require Import notation proofmode.
-From cryptis Require Import lib version term cryptis primitives tactics.
+From iris.heap_lang.lib Require Import ticket_lock.
+From cryptis Require Import lib version term gmeta nown.
+From cryptis Require Import cryptis primitives tactics.
 From cryptis Require Import role dh_auth.
 From cryptis.store Require Import alist db.
 
@@ -12,126 +16,1384 @@ Set Implicit Arguments.
 Unset Strict Implicit.
 Unset Printing Implicit Defensive.
 
-Record cst := {
-  cst_si   :> sess_info;
-  cst_ts   :  loc;
-  cst_name :  gname;
+Record conn_state := ConnState {
+  cs_si   :> sess_info;
+  cs_ts   :  loc;
+  cs_name :  gname;
+  cs_role :  role;
 }.
 
 #[global]
-Instance cst_repr : Repr cst :=
-  λ s, (#(cst_ts s), Spec.mkskey (si_key s))%V.
+Instance cs_repr : Repr conn_state :=
+  λ s, (#(cs_ts s), Spec.mkskey (si_key s))%V.
 
-Record sst := {
-  sst_si  :> sess_info;
-  sst_ts  : loc;
-  sst_db  : loc;
+Record server_state := {
+  ss_key : term;
+  ss_clients : val;
 }.
 
 #[global]
-Instance sst_repr : Repr sst :=
-  λ s, (#(sst_ts s), Spec.mkskey (si_key s), #(sst_db s))%V.
+Instance ss_repr : Repr server_state :=
+  λ s, (TKey Dec (ss_key s), TKey Enc (ss_key s), ss_clients s)%V.
+
+Record server_client_state := {
+  scs_db   : val;
+  scs_name : gname;
+  scs_lock : val;
+}.
+
+#[global]
+Instance scs_repr : Repr server_client_state :=
+  λ s, (scs_db s, scs_lock s)%V.
+
+Section Status.
+
+(**
+
+Each party of the protocol can be in one of two states:
+
+- [Disconnected n] means that the [n] database operations have been performed so
+  far and processed by the server.
+
+- [Connected kS n] means that the participant is connected using the session key
+  [kS] and that, at the beginning of the connection, [n] database operations had
+  been performed.
+
+*)
+
+Variant lstatus :=
+| Disconnected of nat
+| Connected of term & nat.
+
+Canonical lstatusO := leibnizO lstatus.
+
+Global Instance lstatus_inhabited : Inhabited lstatus :=
+  populate (Disconnected inhabitant).
+
+(**
+
+Combining client and server, the system can be in one of four states:
+
+- [BothDisconnected n] means that both parties are disconnected.  If [n = None],
+  then they have never connected to each other; otherwise, [n] indicates how
+  many database operations had been performed previously.
+
+- [ClientConnecting kS n] means that the client is attempting to connected with
+  the server using the session key [kS]. If [n = None], this is the first
+  connection between them; otherwise, [n] is the number of performed database
+  operations.
+
+- [BothConnected kS n] means that the server has accepted the connection of the
+  client.  At this point, we don't need to distinguish between the first and
+  subsequent connection attempts, which is why the number of operations [n] is
+  not optional.
+
+- [ClientDisconnecting kS n] means that the client wants to disconnect the
+  session identified by the key [kS], and that [n] operations have been
+  performed.
+
+*)
+
+Variant gstatus :=
+| BothDisconnected of nat
+| ClientConnecting of term & nat
+| BothConnected of term & nat
+| ClientDisconnecting of term & nat & nat.
+
+Canonical gstatusO := leibnizO gstatus.
+
+Global Instance gstatus_inhabited : Inhabited gstatus :=
+  populate (BothDisconnected inhabitant).
+
+Definition status_view : Type := excl' lstatus.
+
+Implicit Types gs : gstatus.
+Implicit Types ls : lstatus.
+Implicit Types v : status_view.
+Implicit Types n : nat.
+
+Definition to_client_status gs :=
+  match gs with
+  | BothDisconnected n => Disconnected n
+  | ClientConnecting kS n => Connected kS n
+  | BothConnected kS n => Connected kS n
+  | ClientDisconnecting kS beginning ending => Disconnected ending
+  end.
+
+Definition to_server_status gs :=
+  match gs with
+  | BothDisconnected n => Disconnected n
+  | ClientConnecting kS n => Disconnected n
+  | BothConnected kS n => Connected kS n
+  | ClientDisconnecting kS beginning _ => Connected kS beginning
+  end.
+
+Definition to_status gs := Excl' (to_server_status gs).
+
+Definition status_view_rel_raw n gs v :=
+  v ≼ to_status gs.
+
+Lemma status_view_rel_raw_mono n1 n2 gs1 gs2 v1 v2 :
+  status_view_rel_raw n1 gs1 v1 →
+  gs1 ≡{n2}≡ gs2 →
+  v2 ≼{n2} v1 →
+  n2 ≤ n1 →
+  status_view_rel_raw n2 gs2 v2.
+Proof.
+rewrite /status_view_rel_raw.
+move=> v1_gs1 /leibniz_equiv_iff <- {gs2}.
+move=> /cmra_discrete_included_iff v2_v1 n2_n1.
+by trans v1.
+Qed.
+Lemma status_view_rel_raw_valid n gs v :
+  status_view_rel_raw n gs v → ✓{n} v.
+Proof.
+rewrite /status_view_rel_raw => v_gs.
+move: n; apply/cmra_valid_validN.
+apply: cmra_valid_included v_gs.
+by [].
+Qed.
+Lemma status_view_rel_raw_unit n :
+  ∃ gs, status_view_rel_raw n gs ε.
+Proof.
+exists (BothDisconnected 0).
+exact: ucmra_unit_least.
+Qed.
+Canonical Structure status_view_rel : view_rel gstatusO _ :=
+  ViewRel status_view_rel_raw
+    status_view_rel_raw_mono
+    status_view_rel_raw_valid
+    status_view_rel_raw_unit.
+
+Global Instance status_view_rel_discrete : ViewRelDiscrete status_view_rel.
+Proof. by move. Qed.
+
+Notation status := (view status_view_rel).
+
+Definition client_view gs : status :=
+  ●V gs.
+
+Definition server_view ls : status :=
+  ◯V Excl' ls.
+
+Lemma status_valid gs ls :
+  ✓ (client_view gs ⋅ server_view ls) ↔
+  ls = to_server_status gs.
+Proof.
+rewrite view_both_valid /= /status_view_rel_raw /to_status.
+split.
+- move=> /(_ 0). by rewrite Excl_included.
+- by move=> -> _.
+Qed.
+
+Lemma client_connect_update kS n :
+  client_view (BothDisconnected n) ~~> client_view (ClientConnecting kS n).
+Proof.
+apply: (view_update_auth _ _ _ None); rewrite /= /status_view_rel_raw /=.
+move=> _ [ls|_]; last exact: ucmra_unit_least.
+move=> lsE; have ->: ls = Excl (to_server_status (BothDisconnected n)).
+{ rewrite -leibniz_equiv_iff.
+  exact: Some_included_exclusive. }
+exact/Excl_included.
+Qed.
+
+Lemma server_connect_update kS n ls :
+  client_view (ClientConnecting kS n) ⋅ server_view ls ~~>
+  client_view (BothConnected kS n) ⋅ server_view (Connected kS n).
+Proof.
+apply/view_update; rewrite /= /status_view_rel_raw /= => _.
+move=> f incl; have /exclusive_Some_l: ✓ (Excl' ls ⋅ f).
+{ exact: cmra_valid_included incl. }
+by move=> ->; rewrite ucmra_unit_right_id.
+Qed.
+
+Lemma client_disconnect_update kS n ending :
+  client_view (BothConnected kS n) ~~>
+  client_view (ClientDisconnecting kS n ending).
+Proof.
+apply: (view_update_auth _ _ _ None); rewrite /= /status_view_rel_raw /=.
+move=> _ [ls|_]; last exact: ucmra_unit_least.
+move=> lsE; have ->: ls = Excl (to_server_status (BothConnected kS n)).
+{ rewrite -leibniz_equiv_iff.
+  exact: Some_included_exclusive. }
+exact/Excl_included.
+Qed.
+
+Lemma server_disconnect_update kS n ending ls :
+  client_view (ClientDisconnecting kS n ending) ⋅ server_view ls ~~>
+  client_view (BothDisconnected ending) ⋅ server_view (Disconnected ending).
+Proof.
+apply/view_update; rewrite /= /status_view_rel_raw /= => _.
+move=> f incl; have /exclusive_Some_l: ✓ (Excl' ls ⋅ f).
+{ exact: cmra_valid_included incl. }
+by move=> ->; rewrite ucmra_unit_right_id.
+Qed.
+
+End Status.
+
+Notation status := (view status_view_rel_raw).
+Notation statusUR := (viewUR status_view_rel).
+
+Definition oneshotUR : ucmra :=
+  authUR (optionUR (agreeR natO)).
+
+Definition Free dq : oneshotUR :=
+  ●{dq} None.
+
+Definition Shot n : oneshotUR :=
+  ◯ Some (to_agree n).
+
+Lemma shoot n : Free (DfracOwn 1) ~~> Shot n.
+Proof.
+trans (● (Some (to_agree n)) ⋅ Shot n); last first.
+  exact: cmra_update_op_r.
+apply: auth_update_alloc.
+by apply: alloc_option_local_update.
+Qed.
 
 Class storeGS Σ := StoreGS {
-  storeGS_db : dbGS Σ;
+  storeGS_db      : dbGS Σ;
+  storeGS_status  : inG Σ statusUR;
+  storeGS_oneshot : inG Σ oneshotUR
 }.
 
 Local Existing Instance storeGS_db.
+Local Existing Instance storeGS_status.
+Local Existing Instance storeGS_oneshot.
 
-Definition storeΣ := dbΣ.
+Definition storeΣ := #[
+  dbΣ;
+  GFunctor statusUR;
+  GFunctor oneshotUR
+].
 
 Global Instance subG_storeGS Σ : subG storeΣ Σ → storeGS Σ.
 Proof. solve_inG. Qed.
 
 Section Defs.
 
-Context `{!cryptisGS Σ, !heapGS Σ, !storeGS Σ}.
+Context `{!cryptisGS Σ, !heapGS Σ, !storeGS Σ, !tlockG Σ}.
 Notation iProp := (iProp Σ).
 
-Implicit Types (cs : cst) (ss : sst).
+Implicit Types (cs : conn_state).
 Implicit Types kI kR kS t : term.
 Implicit Types db : gmap term term.
+Implicit Types accounts : gmap term server_client_state.
 Implicit Types n : nat.
 Implicit Types b : bool.
-Implicit Types γ : gname.
+Implicit Types γ γ_db γ_s : gname.
 Implicit Types v : val.
-Implicit Types ok : bool.
+Implicit Types ok : Prop.
 Implicit Types si : sess_info.
 
 Variable N : namespace.
 
-Definition client cs : iProp := ∃ (n : nat),
-  session (cst_name cs) cs Init ∗
-  □ (∀ kt, public (TKey kt (si_key cs)) ↔ ▷ session_fail cs) ∗
+Definition dbCN kR := nroot.@"db".@"client".@kR.
+Definition dbSN kI := nroot.@"db".@"server".@kI.
+
+Definition is_conn_state cs n : iProp :=
+  cs_ts cs ↦ #n ∗
+  session (cs_name cs) cs (cs_role cs) ∗
   minted (si_key cs) ∗
-  cst_ts cs ↦ #n ∗
-  DB.client_view (cst_name cs) n.
+  □ (∀ kt, public (TKey kt (si_key cs)) ↔ ▷ session_fail cs).
 
-Definition rem_mapsto cs t1 t2 : iProp :=
-  DB.mapsto (cst_name cs) t1 t2.
+Lemma conn_state_session cs n :
+  is_conn_state cs n -∗
+  session (cs_name cs) cs (cs_role cs).
+Proof. by iIntros "(? & ? & ?)". Qed.
 
-Definition rem_free_at cs T : iProp :=
-  DB.free_at (cst_name cs) T.
+(* MOVE *)
+Definition key_name k γ : iProp :=
+  ∃ c k', ⌜k = Spec.tag c k'⌝ ∗
+          nonce_meta k' nroot γ.
 
-Lemma rem_free_at_diff cs T1 T2 :
+Lemma key_name_agree k γ1 γ2 :
+  key_name k γ1 -∗
+  key_name k γ2 -∗
+  ⌜γ1 = γ2⌝.
+Proof.
+iIntros "(%c1 & %seed1 & -> & #meta1)".
+iIntros "(%c2 & %seed2 & %e & #meta2)".
+case/Spec.tag_inj: e => _ <-.
+iApply (term_meta_agree with "meta1 meta2").
+Qed.
+
+Global Instance key_name_persistent k γ : Persistent (key_name k γ).
+Proof. apply _. Qed.
+
+Global Instance key_name_timeless k γ : Timeless (key_name k γ).
+Proof. apply _. Qed.
+
+Global Typeclasses Opaque key_name.
+(* /MOVE *)
+
+(* MOVE *)
+Definition escrow (N' : namespace) (P Q : iProp) : iProp :=
+  □ (∀ E, ⌜↑N' ⊆ E⌝ -∗ P ={E}=∗ ▷ Q).
+
+Global Typeclasses Opaque escrow.
+
+Global Instance escrow_persistent N' P Q :
+  Persistent (escrow N' P Q).
+Proof. rewrite /escrow. apply _. Qed.
+
+Definition switch (P Q : iProp) : iProp := ∃ R,
+  □ (P ∗ □ R -∗ Q) ∗
+  □ (P ==∗ □ R).
+
+Lemma escrowI (N' : namespace) E (P Q : iProp) :
+  ▷ Q -∗
+  switch P Q ={E}=∗
+  escrow N' P Q.
+Proof.
+rewrite /escrow.
+iIntros "HQ (%R & #contra & #mint)".
+iMod (inv_alloc N' _ (Q ∨ □ R) with "[HQ]") as "#inv".
+{ by eauto. }
+iIntros "!> %E' !> %sub HP".
+iInv "inv" as "[H|#H]".
+- iMod ("mint" with "HP") as "#HR".
+  iModIntro.
+  iSplitL "HR"; first by eauto.
+  by iFrame.
+- iModIntro.
+  iSplitR; first by eauto.
+  iModIntro. iModIntro.
+  by iApply "contra"; eauto.
+Qed.
+
+Lemma escrowE N' P Q E :
+  ↑N' ⊆ E →
+  escrow N' P Q -∗
+  P ={E}=∗
+  ▷ Q.
+Proof.
+rewrite /escrow. iIntros "%sub #e HP".
+iApply "e" => //.
+Qed.
+(* /MOVE *)
+
+Definition db_signed_up kI kR : iProp := ∃ γR,
+  key_name kR γR ∗
+  gmeta γR (dbSN kI) ().
+
+Definition db_not_signed_up kI kR : iProp := ∃ γR,
+  key_name kR γR ∗
+  gmeta_token γR (↑dbSN kI).
+
+Lemma db_signed_up_switch kI kR Q :
+  ⊢ switch (db_not_signed_up kI kR) Q.
+Proof.
+iExists (db_signed_up kI kR). iSplit; iModIntro.
+- iIntros "[no yes]".
+  iDestruct "no" as "(%γR & #name1 & token)".
+  iDestruct "yes" as "(%γR' & #name2 & #meta)".
+  iPoseProof (key_name_agree with "name1 name2") as "->".
+  iDestruct (gmeta_gmeta_token with "token meta") as "[]".
+  solve_ndisj.
+- iIntros "(%γR & #name & token)".
+  iMod (gmeta_set _ _ (dbSN kI) () with "token") as "#meta" => //.
+  iModIntro. iExists γR. iModIntro. by iSplit.
+Qed.
+
+Definition server_status_ready kI kR γI :=
+  escrow (nroot.@"db") (db_not_signed_up kI kR) (
+    nown γI (dbCN kR.@"status") (server_view (Disconnected 0))
+  ).
+
+Definition conn_not_started si rl : iProp := ∃ γ_sR,
+  session γ_sR si rl ∗
+  gmeta_token γ_sR (↑nroot.@"db".@"begin").
+
+Definition conn_started si rl : iProp := ∃ γ_sR,
+  session γ_sR si rl  ∗
+  gmeta γ_sR (nroot.@"db".@"begin") ().
+
+Lemma conn_started_switch si rl Q :
+  ⊢ switch (conn_not_started si rl)
+    (session_fail si ∨ Q).
+Proof.
+iExists (conn_started si rl). iSplit; iModIntro.
+- iIntros "[no #yes]".
+  iDestruct "no" as "(%γ_sR1 & #sess1 & token)".
+  iDestruct "yes" as "(%γ_sR2 & #sess2 & #meta)".
+  iDestruct (session_agree_name with "sess1 sess2") as "[fail|[? ->]]" => //.
+  + by iLeft.
+  + iRight.
+    iDestruct (gmeta_gmeta_token with "token meta") as "[]" => //.
+- iIntros "(%γ_sR & #sess & token)".
+  iMod (gmeta_set _ _ (nroot.@"db".@"begin") () with "token") as "#meta" => //.
+  iIntros "!> !>". iExists _. eauto.
+Qed.
+
+Definition conn_not_ended si rl : iProp := ∃ γ_sR,
+  session γ_sR si rl ∗
+  gmeta_token γ_sR (↑nroot.@"db".@"end").
+
+Definition conn_ended si rl : iProp := ∃ γ_sR,
+  session γ_sR si rl  ∗
+  gmeta γ_sR (nroot.@"db".@"end") ().
+
+Lemma conn_ended_switch si rl Q :
+  ⊢ switch (conn_not_ended si rl) (session_fail si ∨ Q).
+Proof.
+iExists (conn_ended si rl). iSplit; iModIntro.
+- iIntros "[no #yes]".
+  iDestruct "no" as "(%γ_sR1 & #sess1 & token)".
+  iDestruct "yes" as "(%γ_sR2 & #sess2 & #meta)".
+  iDestruct (session_agree_name with "sess1 sess2") as "[fail|[_ ->]]" => //.
+  + by iLeft.
+  + iRight.
+    by iDestruct (gmeta_gmeta_token with "token meta") as "[]".
+- iIntros "(%γ_sR & #sess & token)".
+  iMod (gmeta_set _ _ (nroot.@"db".@"end") () with "token") as "#meta" => //.
+  iIntros "!> !>". iExists _. eauto.
+Qed.
+
+Implicit Types (ls : lstatus) (gs : gstatus).
+
+Definition key_corruption kI kR : iProp :=
+  public (TKey Enc kI) ∨ public (TKey Enc kR).
+
+Definition client_disconnected_int kI kR γI n : iProp :=
+  key_name kI γI ∗
+  DB.client_view γI (dbCN kR.@"state") n ∗
+  server_status_ready kI kR γI ∗
+  (key_corruption kI kR ∨
+   nown γI (dbCN kR.@"status") (client_view (BothDisconnected n))).
+
+Definition client_disconnected kI kR : iProp := ∃ γI n,
+  client_disconnected_int kI kR γI n.
+
+Definition client_connected_int cs γI n beginning : iProp :=
+  let kI := si_init cs in
+  let kR := si_resp cs in
+  ⌜cs_role cs = Init⌝ ∗
+  key_name kI γI ∗
+  DB.client_view γI (dbCN kR.@"state") (n + beginning) ∗
+  server_status_ready kI kR γI ∗
+  conn_not_ended cs Init ∗
+  gmeta (cs_name cs) (nroot.@"db".@"beginning") beginning ∗
+  gmeta_token (cs_name cs) (↑nroot.@"db".@"ending") ∗
+  (session_fail cs ∨
+   nown γI (dbCN kR.@"status")
+     (client_view (BothConnected (si_key cs) beginning))).
+
+Definition client_connecting_int cs γI beginning : iProp :=
+  let kI := si_init cs in
+  let kR := si_resp cs in
+  ⌜cs_role cs = Init⌝ ∗
+  key_name kI γI ∗
+  DB.client_view γI (dbCN kR.@"state") beginning ∗
+  server_status_ready kI kR γI ∗
+  conn_not_started cs Init ∗
+  conn_not_ended cs Init ∗
+  gmeta (cs_name cs) (nroot.@"db".@"beginning") beginning ∗
+  gmeta_token (cs_name cs) (↑nroot.@"db".@"ending").
+
+Definition client_disconnecting_int cs γI n beginning : iProp :=
+  let kI := si_init cs in
+  let kR := si_resp cs in
+  ⌜cs_role cs = Init⌝ ∗
+  key_name kI γI ∗
+  DB.client_view γI (dbCN kR.@"state") (n + beginning) ∗
+  server_status_ready kI kR γI ∗
+  conn_not_ended cs Init ∗
+  gmeta (cs_name cs) (nroot.@"db".@"ending") (n + beginning).
+
+Definition conn_ready si γI n :=
+  escrow (nroot.@"db")
+         (conn_not_started si Resp)
+         (session_fail si ∨
+          nown γI (dbCN (si_resp si).@"status")
+               (client_view (ClientConnecting (si_key si) n))).
+
+Lemma client_connectingI E1 E2 kI kR cs dq n T γI beginning :
+  ↑cryptisN ⊆ E1 →
+  ↑nroot.@"db" ⊆ E1 →
+  ↑nroot.@"db" ⊆ E2 →
+  si_init cs = kI →
+  si_resp cs = kR →
+  si_time cs = n  →
+  cs_role cs = Init →
+  cryptis_ctx -∗
+  £ 1 ∗ £ 1 -∗
+  ●H{dq|n} T -∗
+  is_conn_state cs 0 -∗
+  gmeta_token (cs_name cs) E2 -∗
+  client_disconnected_int kI kR γI beginning ={E1}=∗
+  ●H{dq|n} T ∗
+  is_conn_state cs 0 ∗
+  client_connecting_int cs γI beginning ∗
+  gmeta (cs_name cs) (nroot.@"db".@"beginning") beginning ∗
+  conn_ready cs γI beginning.
+Proof.
+move=> ? ? ? <- <- <- e_rl {kI kR n}.
+iIntros "#? [c1 c2] hon conn token client".
+iPoseProof (conn_state_session with "conn") as "#sess".
+iFrame "conn".
+iDestruct "client" as "(#key_name & client_view & #server & status)".
+iPoseProof (DB.client_view_server_view with "client_view")
+  as "(%db & #server_view)".
+rewrite (gmeta_token_difference _ (↑nroot.@"db".@"begin"));
+  try solve_ndisj.
+iDestruct "token" as "[token' token]".
+iAssert (conn_not_started cs Init)
+  with "[token']" as "not_started".
+{ iExists (cs_name cs). iFrame. rewrite e_rl. eauto. }
+rewrite (gmeta_token_difference _ (↑nroot.@"db".@"end")); try solve_ndisj.
+iDestruct "token" as "[token' token]".
+iAssert (conn_not_ended cs Init) with "[token']" as "not_ended".
+{ iExists (cs_name cs). iFrame. rewrite e_rl. eauto. }
+iMod (gmeta_set' _ _ (nroot.@"db".@"beginning") beginning with "token")
+  as "[#beginning token]"; try solve_ndisj.
+iPoseProof (@gmeta_token_drop _ _ (↑nroot.@"db".@"ending") with "token")
+  as "token"; try solve_ndisj.
+iAssert (|={E1}=> ●H{dq|si_time cs} T ∗ (
+                      session_fail cs ∨
+                      nown γI (dbCN (si_resp cs).@"status")
+                        (client_view (ClientConnecting (si_key cs) beginning))))%I
+  with "[c1 hon status]" as ">[hon status]".
+{ iDestruct "status" as "[#fail|status]".
+  - iAssert (|={E1}=> ●H{dq|si_time cs} T ∗ session_fail cs)%I
+    with "[c1 hon]"
+    as ">[hon #fail']".
+    { iDestruct "fail" as "[fail|fail]".
+      - iMod (public_atI with "[//] c1 hon fail") as "{fail} [hon fail]".
+        { solve_ndisj. }
+        by iFrame.
+      - iMod (public_atI with "[//] c1 hon fail") as "{fail} [hon fail]".
+        { solve_ndisj. }
+        by iFrame. }
+    iFrame.
+    by iLeft.
+  - iFrame.
+    iMod (nown_update with "status") as "status".
+    { apply: (client_connect_update (si_key cs)). }
+    iModIntro. by iRight. }
+iAssert (|={E1}=> conn_ready cs γI beginning)%I with "[status]" as ">#ready".
+{ iApply (escrowI with "status").
+  iApply conn_started_switch. }
+iFrame "hon". iSplitL => //; eauto.
+iFrame. by eauto.
+Qed.
+
+Definition conn_accepted si γI beginning :=
+  escrow (nroot.@"db")
+    (conn_not_started si Init)
+    (session_fail si ∨
+     nown γI (dbCN (si_resp si).@"status")
+       (client_view (BothConnected (si_key si) beginning))).
+
+Lemma client_connected_intI cs γI beginning E :
+  ↑nroot.@"db" ⊆ E →
+  client_connecting_int cs γI beginning -∗
+  session_fail cs ∨
+    conn_accepted cs γI beginning ={E}=∗
+  ▷ client_connected_int cs γI 0 beginning.
+Proof.
+move=> sub.
+iIntros "(%e_rl & #name & client & #server & not_started & not_ended &
+          #beginning & ending) #status".
+iFrame. do 4!iSplitR => //.
+iDestruct "status" as "[fail|accepted]".
+- by eauto.
+- iMod (escrowE with "accepted not_started") as "status" => //.
+Qed.
+
+Definition client_connected kI kR cs : iProp := ∃ γI n beginning,
+  ⌜si_init cs = kI⌝ ∗
+  ⌜si_resp cs = kR⌝ ∗
+  is_conn_state cs n ∗
+  client_connected_int cs γI n beginning.
+
+Definition rem_mapsto kI kR t1 t2 : iProp := ∃ γI,
+  key_name kI γI ∗
+  DB.mapsto γI (dbCN kR.@"state") t1 t2.
+
+Lemma rem_mapsto_open kI kR t1 t2 γI :
+  rem_mapsto kI kR t1 t2 -∗
+  key_name kI γI -∗
+  DB.mapsto γI (dbCN kR.@"state") t1 t2 ∗
+  (DB.mapsto γI (dbCN kR.@"state") t1 t2 -∗
+   rem_mapsto kI kR t1 t2).
+Proof.
+iIntros "(%γI' & #name' & mapsto) #name".
+iPoseProof (key_name_agree with "name name'") as "->".
+iFrame. iIntros "?". iExists _. by iFrame.
+Qed.
+
+Definition rem_free_at kI kR T : iProp := ∃ γI,
+  key_name kI γI ∗
+  DB.free_at γI (dbCN kR.@"state") T.
+
+Lemma rem_free_at_diff kI kR T1 T2 :
   T1 ⊆ T2 →
-  rem_free_at cs T2 ⊣⊢ rem_free_at cs T1 ∗ rem_free_at cs (T2 ∖ T1).
-Proof. exact: DB.free_at_diff. Qed.
+  rem_free_at kI kR T2 ⊣⊢ rem_free_at kI kR T1 ∗ rem_free_at kI kR (T2 ∖ T1).
+Proof.
+iIntros "%sub". iSplit.
+- iIntros "(%γI & #name & free)".
+  rewrite (DB.free_at_diff _ _ sub).
+  iDestruct "free" as "[free1 free2]".
+  by iSplitL "free1"; iExists _; iFrame.
+- iIntros "[(%γI1 & #name1 & free1) (%γI2 & #name2 & free2)]".
+  iPoseProof (key_name_agree with "name1 name2") as "->".
+  iExists γI2. iSplit => //.
+  rewrite (DB.free_at_diff _ _ sub). iFrame.
+Qed.
 
-Definition server ss : iProp := ∃ γ (n : nat) kvs db,
-  session γ ss Resp ∗
-  □ (∀ kt, public (TKey kt (si_key ss)) ↔ ▷ session_fail ss) ∗
-  minted (si_key ss) ∗
-  sst_ts ss ↦ #n ∗
-  sst_db ss ↦ kvs ∗
-  ⌜AList.is_alist kvs (repr <$> db)⌝ ∗
-  ([∗ map] t1 ↦ t2 ∈ db, public t1 ∗ public t2) ∗
-  (session_fail ss ∨
-   ∃ γ', session γ' ss Init ∗ DB.server_view γ' n db).
+Lemma rem_mapsto_update t2' cs γI t1 t2 n beginning :
+  is_conn_state cs n -∗
+  client_connected_int cs γI n beginning -∗
+  rem_mapsto (si_init cs) (si_resp cs) t1 t2 ==∗
+  client_connected_int cs γI (S n) beginning ∗
+  is_conn_state cs n ∗
+  rem_mapsto (si_init cs) (si_resp cs) t1 t2' ∗
+  DB.update_at γI (dbCN (si_resp cs).@"state") (n + beginning) t1 t2'.
+Proof.
+iIntros "conn (%e_rl & #name & client & #server & not_ended &
+          #beginning & ending & status)".
+iPoseProof (conn_state_session with "conn") as "#sessI". iFrame "conn".
+iIntros "(%γI' & #name' & mapsto)".
+iPoseProof (key_name_agree with "name' name") as "{name'} ->".
+iMod (DB.update_client t2' with "client mapsto")
+  as "(client & #update & mapsto)".
+iFrame.
+iSplitR.
+{ iFrame. eauto. }
+iSplitL.
+{ iExists γI. iFrame. eauto. }
+by eauto.
+Qed.
 
-Definition init_pred kS (m : term) : iProp := ∃ si γ,
+Lemma rem_mapsto_alloc cs γI t1 t2 n beginning T :
+  t1 ∈ T →
+  is_conn_state cs n -∗
+  client_connected_int cs γI n beginning -∗
+  rem_free_at (si_init cs) (si_resp cs) T ==∗
+  is_conn_state cs n ∗
+  client_connected_int cs γI (S n) beginning ∗
+  rem_mapsto (si_init cs) (si_resp cs) t1 t2 ∗
+  rem_free_at (si_init cs) (si_resp cs) (T ∖ {[t1]}) ∗
+  DB.create_at γI (dbCN (si_resp cs).@"state") (n + beginning) t1 t2.
+Proof.
+iIntros "%t1_T".
+iIntros "conn (%e_rl & #name & client & #server & not_ended &
+          #beginning & ending & status)".
+iPoseProof (conn_state_session with "conn") as "#sessI". iFrame "conn".
+have {}t1_T : {[t1]} ⊆ T by set_solver.
+rewrite (rem_free_at_diff _ _ t1_T).
+iIntros "[(%γI' & #name' & free) free']". iFrame "free'".
+iPoseProof (key_name_agree with "name' name") as "{name'} ->".
+iMod (DB.create_client _ t2 with "client free") as "(create & client & mapsto)".
+iFrame. iModIntro.
+iSplitR.
+{ iFrame. by eauto. }
+iExists γI. by iFrame.
+Qed.
+
+Lemma client_alloc kI kR γI E E' :
+  ↑dbCN kR ⊆ E →
+  ↑nroot.@"db" ⊆ E' →
+  key_name kI γI -∗
+  gmeta_token γI E ={E'}=∗
+  client_disconnected kI kR ∗
+  rem_free_at kI kR ⊤ ∗
+  gmeta_token γI (E ∖ ↑dbCN kR).
+Proof.
+iIntros "%sub %sub' #kI_γI kI_token".
+rewrite (gmeta_token_difference _ _ _ sub).
+iDestruct "kI_token" as "[kI_token ?]". iFrame.
+iMod (DB.alloc _ (N := dbCN kR.@"state") with "kI_token")
+  as "(client_view & free & #server_view & kI_token)".
+{ solve_ndisj. }
+iMod (nown_alloc (dbCN kR.@"status")
+        (client_view (BothDisconnected 0) ⋅ server_view (Disconnected 0))
+  with "kI_token") as "[[client server] kI_token]" => //.
+- solve_ndisj.
+- exact/status_valid.
+iAssert (|={E'}=> server_status_ready kI kR γI)%I
+  with "[server]" as ">#server".
+{ iApply (escrowI with "server").
+  iApply db_signed_up_switch. }
+iModIntro. iSplitR "free".
+- iExists γI, 0. iFrame. iSplit => //.
+- iExists γI. by iFrame.
+Qed.
+
+Definition public_db db : iProp :=
+  [∗ map] t1 ↦ t2 ∈ db, public t1 ∗ public t2.
+
+Lemma public_db_insert db t1 t2 :
+  public t1 -∗
+  public t2 -∗
+  public_db db -∗
+  public_db (<[t1 := t2]> db).
+Proof.
+rewrite /public_db !big_sepM_forall.
+iIntros "#p_t1 #p_t2 #p_db %t1' %t2'".
+case: (decide (t1' = t1)) => [-> {t1'} | ne].
+- rewrite lookup_insert. iIntros "%e". case: e => ->. by eauto.
+- by rewrite lookup_insert_ne //.
+Qed.
+
+Definition server_connected cs n db : iProp :=
+  ⌜cs_role cs = Resp⌝ ∗
+  conn_not_ended cs Resp ∗
+  public_db db ∗
+  (session_fail cs ∨ ∃ γI γ_sI beginning,
+   key_name (si_init cs) γI ∗
+   session γ_sI cs Init ∗
+   DB.server_view γI (dbCN (si_resp cs).@"state") (n + beginning) db ∗
+   gmeta γ_sI (nroot.@"db".@"beginning") beginning ∗
+   nown γI (dbCN (si_resp cs).@"status")
+     (server_view (Connected (si_key cs) beginning))).
+
+Definition server_disconnected kI kR db : iProp :=
+  public_db db ∗
+  (key_corruption kI kR ∨
+   ⌜db = ∅⌝ ∗ db_not_signed_up kI kR ∨ ∃ γI n,
+   key_name kI γI ∗
+   DB.server_view γI (dbCN kR.@"state") n db ∗
+   nown γI (dbCN kR.@"status") (server_view (Disconnected n))).
+
+Definition server_connecting cs db : iProp :=
+  public_db db ∗
+  (session_fail cs ∨
+   ⌜db = ∅⌝ ∗ db_not_signed_up (si_init cs) (si_resp cs) ∨ ∃ γI n,
+   key_name (si_init cs) γI ∗
+   DB.server_view γI (dbCN (si_resp cs).@"state") n db ∗
+   nown γI (dbCN (si_resp cs).@"status") (server_view (Disconnected n))).
+
+Lemma server_connectingI cs db dq T :
+  cryptis_ctx -∗
+  ●H{dq|si_time cs} T -∗
+  £ 1 -∗
+  server_disconnected (si_init cs) (si_resp cs) db ={⊤}=∗
+  ●H{dq|si_time cs} T ∗
+  server_connecting cs db.
+Proof.
+iIntros "#ctx hon c (#p_db & [#fail | status])"; last first.
+{ iModIntro. by iFrame. }
+iAssert (|={⊤}=> ●H{dq|si_time cs} T ∗ session_fail cs)%I
+  with "[hon c]" as "{fail} >[hon fail]".
+{ iDestruct "fail" as "[fail|fail]".
+  - iMod (public_atI with "[//] c hon fail") as "[hon ?]" => //.
+    iModIntro. by iFrame.
+  - iMod (public_atI with "[//] c hon fail") as "[hon ?]" => //.
+    iModIntro. by iFrame. }
+iModIntro. by iFrame.
+Qed.
+
+Definition account_inv kI kR vdb : iProp := ∃ db,
+  server_disconnected kI kR db ∗
+  SAList.is_alist vdb (repr <$> db).
+
+Lemma account_alloc kI kR γR vdb E :
+  ↑dbSN kI ⊆ E →
+  key_name kR γR -∗
+  gmeta_token γR E -∗
+  SAList.is_alist vdb ∅ -∗
+  gmeta_token γR (E ∖ ↑dbSN kI) ∗
+  account_inv kI kR vdb.
+Proof.
+iIntros "%sub #name token vdb".
+rewrite (gmeta_token_difference γR (↑dbSN kI)) //.
+iDestruct "token" as "[token H]". iFrame "H".
+iExists ∅. iFrame "vdb".
+iSplit; first by rewrite /public_db big_sepM_empty.
+iRight. iLeft. iSplit => //. iExists γR. by iFrame.
+Qed.
+
+Definition server ss : iProp := ∃ γR accounts E,
+  public (TKey Dec (ss_key ss)) ∗
+  SAList.is_alist (ss_clients ss) (repr <$> accounts) ∗
+  key_name (ss_key ss) γR ∗
+  gmeta_token γR E ∗
+  ⌜∀ kI, TKey Dec kI ∉ dom accounts → ↑dbSN kI ⊆ E⌝ ∗
+  [∗ map] vkI ↦ scs ∈ accounts, ∃ kI, ⌜vkI = TKey Dec kI⌝ ∗
+     is_lock (scs_name scs) (scs_lock scs)
+       (account_inv kI (ss_key ss) (scs_db scs)).
+
+Lemma serverI kR γR vclients :
+  key_name kR γR -∗
+  gmeta_token γR (↑nroot.@"db".@"server") -∗
+  public (TKey Dec kR) -∗
+  SAList.is_alist vclients ∅ -∗
+  server {| ss_key := kR; ss_clients := vclients |}.
+Proof.
+iIntros "#name token #p_vk clients".
+iExists γR, ∅, (↑nroot.@"db".@"server") => /=.
+iFrame. iSplit => //. iSplit => //. iSplit.
+- iPureIntro. move=> *. solve_ndisj.
+- by rewrite big_sepM_empty.
+Qed.
+
+Definition init_pred kS (m : term) : iProp := ∃ γI si γ_sI (beginning : nat),
   ⌜si_key si = kS⌝ ∗
-  session γ si Init ∗
-  DB.server_view γ 0 ∅.
+  key_name (si_init si) γI ∗
+  session γ_sI si Init ∗
+  gmeta γ_sI (nroot.@"db".@"beginning") beginning ∗
+  server_status_ready (si_init si) (si_resp si) γI ∗
+  conn_ready si γI beginning ∗
+  DB.server_view γI (dbCN (si_resp si).@"state") 0 ∅.
 
-Definition store_pred kS m : iProp := ∃ (n : nat) t1 t2 si γ,
+Lemma init_predI cs γI beginning m :
+  is_conn_state cs 0 -∗
+  client_connecting_int cs γI beginning -∗
+  conn_ready cs γI beginning -∗
+  is_conn_state cs 0 ∗
+  client_connecting_int cs γI beginning ∗
+  □ init_pred (si_key cs) m.
+Proof.
+iIntros "conn (%e_rl & #name & client & #server & not_started & not_ended &
+          #beginning & ending) #ready".
+iPoseProof (DB.client_view_server_view with "client")
+  as "(%db & #server_view)".
+iPoseProof (DB.server_view_to_0 with "server_view") as "#server_view0".
+iPoseProof (conn_state_session with "conn") as "#sessI".
+iFrame. iSplit; first by eauto.
+iModIntro. iExists γI, cs, (cs_name cs), beginning. rewrite e_rl.
+by eauto 10.
+Qed.
+
+Definition ack_init_pred kS (m : term) : iProp := ∃ γ_sR si,
+  ⌜si_key si = kS⌝ ∗
+  session γ_sR si Resp ∗
+  (session_fail si ∨ ∃ γI γ_sI beginning,
+   key_name (si_init si) γI ∗
+   session γ_sI si Init ∗
+   gmeta γ_sI (nroot.@"db".@"beginning") beginning ∗
+   conn_accepted si γI beginning).
+
+Lemma ack_init_predI cs db m :
+  cs_role cs = Resp →
+  server_connecting cs db -∗
+  is_conn_state cs 0 -∗
+  conn_not_started cs Resp -∗
+  conn_not_ended cs Resp -∗
+  (session_fail cs ∗ public m ∨ init_pred (si_key cs) m) ={⊤}▷=∗
+  is_conn_state cs 0 ∗
+  server_connected cs 0 db ∗
+  □ ack_init_pred (si_key cs) (TInt 0).
+Proof.
+iIntros "%e_rl (#p_db & status) conn not_started not_ended p_m".
+iPoseProof (conn_state_session with "conn") as "#sessR".
+iFrame "conn".
+iAssert (□ (▷ session_fail cs -∗ conn_not_ended cs Resp ={⊤}▷=∗
+            server_connected cs 0 db ∗
+            □ ack_init_pred (si_key cs) (TInt 0)))%I
+  as "failure".
+{ iIntros "!> #fail not_ended !> !> !>". iSplit.
+  - by iFrame; eauto.
+  - iModIntro. iExists _, _. rewrite e_rl.
+    iSplit => //. iSplit => //.
+    by iLeft. }
+iDestruct "p_m" as "[[#fail _]|p_m]".
+{ by iApply ("failure" with "[//] not_ended"). }
+iDestruct "status" as "[#fail|status]".
+{ by iApply ("failure" with "[//] not_ended"). }
+iDestruct "p_m"
+  as "(%γI & %si & %γ_sI & %beginning & %e_kS & #name & #sessI &
+       #beginning & #server & #conn_ready & #server_view)".
+iDestruct (session_agree with "sessI sessR") as "[#fail|->]" => //.
+{ by iApply ("failure" with "[//] not_ended"). }
+iMod (escrowE with "conn_ready not_started") as "[#fail|statusI]" => //.
+{ by iApply ("failure" with "[//] not_ended"). }
+iAssert (|={⊤}▷=> ∃ n, DB.server_view γI (dbCN (si_resp cs).@"state") n db ∗
+                         nown γI (dbCN (si_resp cs).@"status")
+                         (server_view (Disconnected n)))%I
+  with "[status]" as ">status".
+{ iDestruct "status" as "[[-> fresh]|status]"; last first.
+  { iDestruct "status" as "(%γI' & %n & #name' & #server_view' & status)".
+    iPoseProof (key_name_agree with "name' name") as "{name'} ->".
+    iIntros "!> !> !>". iExists n. by iFrame. }
+  iMod (escrowE with "server fresh") as "status" => //.
+  iIntros "!> !> !>". iExists 0.  by iFrame. }
+iIntros "!> !>".
+iMod "status" as "(%n & #? & status)".
+iPoseProof (nown_valid_2 with "statusI status") as "%valid".
+case/status_valid: valid => -> {n}.
+iMod (nown_update_2 with "statusI status") as "[statusI status]".
+{ apply: server_connect_update. }
+iAssert (|={⊤}=> conn_accepted cs γI beginning)%I
+  with "[statusI]" as ">#accepted".
+{ iApply (escrowI with "[statusI]"); first by iFrame.
+  iApply conn_started_switch. }
+iModIntro. iSplit.
+{ iFrame. do 2!iSplit => //. iRight.
+  iExists _, _, _. iFrame. by eauto. }
+iIntros "!>". iExists _, _. iSplit => //.
+rewrite e_rl. iSplit => //. iRight.
+iExists _, _, _. by eauto.
+Qed.
+
+Lemma ack_init_predE cs m γI beginning E :
+  ↑nroot.@"db" ⊆ E →
+  is_conn_state cs 0 -∗
+  client_connecting_int cs γI beginning -∗
+  (session_fail cs ∗ public m ∨ ack_init_pred (si_key cs) m) ={E}=∗
+  is_conn_state cs 0 ∗
+  ▷ client_connected_int cs γI 0 beginning.
+Proof.
+iIntros "%sub conn".
+iIntros "(%e_rl & #name & client & #server & not_started & not_ended &
+          #beginning & ending) m".
+iPoseProof (conn_state_session with "conn") as "#sess". iFrame "conn".
+iAssert (|={E}=> ▷ (session_fail cs ∨
+                    nown γI (dbCN (si_resp cs).@"status")
+                        (client_view (BothConnected (si_key cs) beginning))))%I
+  with "[not_started m]" as ">status".
+{ iDestruct "m" as "[[m _]|m]"; eauto.
+  iDestruct "m" as "(%γ_sR & %si & %e_kS & #sess' & m)".
+  iDestruct (session_agree with "sess' sess") as "[fail|->]" => //.
+  { by iLeft. }
+  iDestruct "m" as "[fail|m]".
+  { by iLeft. }
+  iDestruct "m" as "(%γI' & %γ_sI & %beginning' & #name' & #sess'' & #beginning' &
+                     #accepted)".
+  rewrite e_rl.
+  iDestruct (session_agree_name with "sess sess''") as "[fail|[_ <-]]" => //.
+  { by iLeft. }
+  iMod (escrowE with "accepted not_started") as "status" => //.
+  eauto.
+  iPoseProof (key_name_agree with "name name'") as "<-".
+  by iPoseProof (gmeta_agree with "beginning beginning'") as "->". }
+do !iModIntro.
+iFrame. eauto.
+Qed.
+
+Definition store_pred kS m : iProp := ∃ (n : nat) t1 t2 si γI γ beginning,
   ⌜m = Spec.of_list [TInt n; t1; t2]⌝ ∗
   ⌜si_key si = kS⌝ ∗
   session γ si Init ∗
+  key_name (si_init si) γI ∗
   public t1 ∗
   public t2 ∗
-  DB.update_at γ n t1 t2.
+  gmeta γ (nroot.@"db".@"beginning") beginning ∗
+  DB.update_at γI (dbCN (si_resp si).@"state") (n + beginning) t1 t2.
+
+Lemma store_predI cs γI n beginning t1 t2 :
+  is_conn_state cs (S n) -∗
+  client_connected_int cs γI (S n) beginning -∗
+  public t1 -∗
+  public t2 -∗
+  DB.update_at γI (dbCN (si_resp cs).@"state") (n + beginning) t1 t2 -∗
+  is_conn_state cs (S n) ∗
+  client_connected_int cs γI (S n) beginning ∗
+  □ store_pred (si_key cs) (Spec.of_list [TInt n; t1; t2]).
+Proof.
+iIntros "conn (%e_rl & #name & client & #server & not_ended &
+          #beginning & ending & status)".
+iPoseProof (conn_state_session with "conn") as "#sessI". iFrame "conn".
+iIntros "#p_t1 #p_t2 #update".
+iFrame. iSplit; first by eauto.
+iModIntro. iExists n, t1, t2, cs, γI, (cs_name cs), beginning. rewrite e_rl.
+by eauto 10.
+Qed.
+
+Lemma store_predE cs n db t1 t2 :
+  let m := Spec.of_list [TInt n; t1; t2] in
+  is_conn_state cs n -∗
+  server_connected cs n db -∗
+  session_fail cs ∗ public m ∨ store_pred (si_key cs) m -∗
+  is_conn_state cs n ∗
+  server_connected cs (S n) (<[t1 := t2]>db).
+Proof.
+iIntros "%m conn server m_inv".
+iPoseProof (conn_state_session with "conn") as "#sessR".
+iFrame "conn".
+iDestruct "server" as "(%e_rl & not_ended & #p_db & status)".
+iFrame "not_ended".
+iSplit => //.
+iDestruct "m_inv" as "[[#fail #p_m]|m_inv]".
+{ rewrite public_of_list /=.
+  iDestruct "p_m" as "(_ & p_t1 & p_t2 & _)".
+  iSplitR; last by eauto.
+  by iApply public_db_insert. }
+iDestruct "m_inv"
+  as "(%n' & %t1' & %t2' & %si & %γI & %γ_sI & %beginning &
+      %e_m & %e_kS & #sessI & #name & #p_t1 & #p_t2 &
+      #beginning & #update)".
+case/Spec.of_list_inj: e_m => e_n <- <- {t1' t2'}.
+have {e_n} <- : n = n' by lia.
+iSplit.
+{ by iApply public_db_insert. }
+iDestruct "status" as "[#fail|status]"; first by eauto.
+iDestruct "status"
+  as "(%γI' & %γ_sI' & %beginning' & #name' & #sessI' &
+       #server & #beginning' & status)".
+iPoseProof (session_agree with "sessI sessR") as "[fail|->]" => //.
+{ by eauto. }
+iPoseProof (session_agree_name with "sessI' sessI") as "[fail|[_ ->]]" => //.
+{ by eauto. }
+iPoseProof (key_name_agree with "name' name") as "{name' sessI'} ->".
+iPoseProof (gmeta_agree with "beginning' beginning") as "{beginning'} ->".
+iPoseProof (DB.update_server with "server update") as "{server} server".
+iRight. iExists _, _, _. iFrame.
+do !iSplit => //.
+Qed.
 
 Definition ack_store_pred kS m : iProp := ∃ (n : nat),
   ⌜m = TInt n⌝. (* FIXME: Do we need anything else here? *)
 
 Definition load_pred (kS m : term) : iProp := True.
 
-Definition ack_load_pred (kS m : term) : iProp := ∃ n t1 t2 si γ,
+Definition ack_load_pred (kS m : term) : iProp := ∃ n t1 t2 γ si,
   ⌜m = Spec.of_list [TInt n; t1; t2]⌝ ∗
   ⌜si_key si = kS⌝ ∗
   public t2 ∗
   session γ si Resp ∗
-  (session_fail si ∨ ∃ γ', session γ' si Init ∗ DB.stored_at γ' n t1 t2).
+  (session_fail si ∨ ∃ γI γ' beginning,
+   key_name (si_init si) γI ∗
+   session γ' si Init ∗
+   gmeta γ' (nroot.@"db".@"beginning") beginning ∗
+   DB.stored_at γI (dbCN (si_resp si).@"state") (n + beginning) t1 t2).
 
-Definition create_pred kS m : iProp := ∃ n t1 t2 si γ,
+
+Lemma ack_load_predI {cs n db t1 t2} :
+  db !! t1 = Some t2 →
+  is_conn_state cs n -∗
+  server_connected cs n db -∗
+  public (Spec.of_list [TInt n; t1; t2]) ∗
+  □ ack_load_pred (si_key cs) (Spec.of_list [TInt n; t1; t2]).
+Proof.
+iIntros "%t1_t2 conn server".
+iPoseProof (conn_state_session with "conn") as "#sessR".
+iDestruct "server" as "(%e_rl & not_ended & #public & status)".
+rewrite /public_db big_sepM_forall.
+iDestruct ("public" with "[//]") as "[p_t1 p_t2]".
+iSplit.
+{ rewrite public_of_list /= public_TInt. by eauto. }
+rewrite e_rl. iExists n, t1, t2, (cs_name cs), cs.
+do !iSplitR => //.
+iDestruct "status" as "[#fail|status]"; first by eauto.
+iDestruct "status"
+  as "(%γI & %γ_sI & %beginning & #name & #sessI & #server & #beginning & _)".
+iPoseProof (DB.load_server _ _ _ t1_t2 with "server") as "#load".
+iModIntro. iRight. iExists _, _, _. by eauto.
+Qed.
+
+Lemma ack_loadE cs γI n beginning t1 t2 t2' :
+  let m := Spec.of_list [TInt n; t1; t2'] in
+  is_conn_state cs n -∗
+  client_connected_int cs γI n beginning -∗
+  rem_mapsto (si_init cs) (si_resp cs) t1 t2 -∗
+  □ (session_fail cs ∗ public m ∨ ack_load_pred (si_key cs) m) -∗
+  is_conn_state cs n ∗
+  client_connected_int cs γI n beginning ∗
+  rem_mapsto (si_init cs) (si_resp cs) t1 t2 ∗
+  public t2' ∗
+  (session_fail cs ∨ ⌜t2' = t2⌝).
+Proof.
+iIntros "conn (%e_rl & #name & client & #server & not_ended &
+          #beginning & ending & status)".
+iPoseProof (conn_state_session with "conn") as "#sessI". iFrame "conn".
+iIntros "mapsto".
+iIntros "[[#fail p_m]|p_m]".
+{ rewrite public_of_list /=. iDestruct "p_m" as "(_ & _ & p_t2' & _)".
+  iFrame. iSplit; eauto. }
+iDestruct "mapsto" as "(%γI' & #name' & mapsto)".
+iPoseProof (key_name_agree with "name' name") as "{name'} ->".
+iDestruct "p_m"
+  as "#(%n' & %t1' & %t2'' & %γ & %si & %e & %e_key & #p_t2' & #sessR & r)".
+case/Spec.of_list_inj: e => e_n <- <- {t1' t2''}.
+have {n' e_n} <-: n = n' by lia.
+rewrite (assoc bi_sep). iSplit.
+{ iSplitR "mapsto".
+  { iFrame. by eauto. }
+  iExists _. by iFrame. }
+iSplit => //.
+iPoseProof (session_agree with "sessR sessI") as "[fail|->]" => //.
+{ by iLeft. }
+iDestruct "r" as "[fail|r]"; first by iLeft.
+iDestruct "r"
+  as "(%γI' & %γ' & %beginning' & #name' & #sessI' & #beginning' & #stored)".
+iPoseProof (key_name_agree with "name' name") as "{name'} ->".
+rewrite e_rl.
+iPoseProof (session_agree_name with "sessI' sessI") as "[fail|[_ ->]]" => //.
+{ by iLeft. }
+iPoseProof (gmeta_agree with "beginning' beginning") as "{beginning'} ->".
+iRight.
+by iApply (DB.load_client with "client mapsto stored").
+Qed.
+
+Definition create_pred kS m : iProp := ∃ n t1 t2 si γI γ beginning,
   ⌜m = Spec.of_list [TInt n; t1; t2]⌝ ∗
   ⌜si_key si = kS⌝ ∗
+  key_name (si_init si) γI ∗
   session γ si Init ∗
+  gmeta γ (nroot.@"db".@"beginning") beginning ∗
   public t1 ∗
   public t2 ∗
-  DB.create_at γ n t1 t2.
+  DB.create_at γI (dbCN (si_resp si).@"state") (n + beginning) t1 t2.
+
+Lemma create_predI cs n m t1 t2 γI beginning :
+  is_conn_state cs m -∗
+  client_connected_int cs γI (S n) beginning -∗
+  public t1 -∗
+  public t2 -∗
+  DB.create_at γI (dbCN (si_resp cs).@"state") (n + beginning) t1 t2 -∗
+  is_conn_state cs m ∗
+  client_connected_int cs γI (S n) beginning ∗
+  □ create_pred (si_key cs) (Spec.of_list [TInt n; t1; t2]).
+Proof.
+iIntros "conn (%e_rl & #name & client & #server & not_ended &
+          #beginning & ending & status)".
+iPoseProof (conn_state_session with "conn") as "#sessI". iFrame "conn".
+iIntros "#p_t1 #p_t2 #create".
+iFrame.
+iSplit; first by eauto.
+iExists n, t1, t2, cs, γI, (cs_name cs), beginning. rewrite e_rl.
+by eauto 10.
+Qed.
+
+Lemma public_create_pred cs n t1 t2 :
+  let m := Spec.of_list [TInt n; t1; t2] in
+  (session_fail cs ∗ public m ∨ create_pred (si_key cs) m) -∗
+  public t1 ∗ public t2.
+Proof.
+iIntros "[[_ p_m]|m_inv]".
+- rewrite public_of_list /=.
+  iDestruct "p_m" as "(_ & p_t1 & p_t2 & _)".
+  by eauto.
+- iDestruct "m_inv"
+    as "(%n' & %t1' & %t2' & %si & %γI & %γ_sI & %beginning &
+       %e_m & %e_kS & #name & #sessI & #beginning & #p_t1 & #p_t2 &
+       #created)".
+  case/Spec.of_list_inj: e_m => e_n <- <- {t1' t2'}.
+  by eauto.
+Qed.
+
+Lemma create_predE cs n db t1 t2 :
+  let m := Spec.of_list [TInt n; t1; t2] in
+  db !! t1 = None →
+  is_conn_state cs n -∗
+  server_connected cs n db -∗
+  (session_fail cs ∗ public m ∨ create_pred (si_key cs) m) -∗
+  is_conn_state cs n ∗
+  server_connected cs (S n) (<[t1 := t2]> db).
+Proof.
+iIntros "%m %db_t1 conn server m_inv".
+iPoseProof (conn_state_session with "conn") as "#sessR".
+iFrame "conn".
+iDestruct "server" as "(%e_rl & not_ended & #p_db & status)".
+iFrame. iSplitR => //.
+iDestruct "m_inv" as "[[#fail #p_m] | m_inv]".
+{ rewrite public_of_list /=.
+  iDestruct "p_m" as "(_ & p_t1 & p_t2 & _)".
+  iSplitR; last by eauto.
+  by iApply public_db_insert. }
+iDestruct "m_inv"
+  as "(%n' & %t1' & %t2' & %si & %γI & %γ_sI & %beginning &
+       %e_m & %e_kS & #name & #sessI & #beginning & #p_t1 & #p_t2 &
+       #created)".
+case/Spec.of_list_inj: e_m => e_n <- <- {t1' t2'}.
+have {n' e_n} <- : n = n' by lia.
+iSplitR.
+{  by iApply public_db_insert. }
+iDestruct "status" as "[#fail | status]"; first by iLeft.
+iDestruct "status"
+  as "(%γI' & %γ_sI' & %beginning' & #name' & #sessI' & #server &
+       #beginning' & status)".
+iPoseProof (session_agree_name with "sessI sessI'") as "[fail |[-> <-]]" => //.
+{ by iLeft. }
+iClear "sessI'".
+iPoseProof (key_name_agree with "name' name") as "{name'} ->".
+iPoseProof (gmeta_agree with "beginning' beginning") as "{beginning'} ->".
+iPoseProof (DB.create_server with "server created") as "{server} server" => //.
+iRight.
+iExists _, _, _. iFrame. by eauto.
+Qed.
 
 Definition ack_create_pred kS (m : term) : iProp := True.
 
+Definition conn_done si γI beginning ending :=
+  escrow (nroot.@"db")
+         (conn_not_ended si Resp)
+         (session_fail si ∨
+            nown γI (dbCN (si_resp si).@"status")
+                 (client_view (ClientDisconnecting (si_key si) beginning ending))).
+
+Definition close_pred kS m : iProp := ∃ n si γI γ beginning,
+  ⌜m = TInt n⌝ ∗
+  ⌜si_key si = kS⌝ ∗
+  key_name (si_init si) γI ∗
+  session γ si Init ∗
+  gmeta γ (nroot.@"db".@"beginning") beginning ∗
+  gmeta γ (nroot.@"db".@"ending") (n + beginning) ∗
+  conn_done si γI beginning (n + beginning).
+
+Lemma close_predI cs γI beginning n E :
+  ↑nroot.@"db" ⊆ E →
+  is_conn_state cs n -∗
+  client_connected_int cs γI n beginning ={E}=∗
+  is_conn_state cs n ∗
+  client_disconnecting_int cs γI n beginning ∗
+  □ close_pred (si_key cs) (TInt n).
+Proof.
+iIntros "%sub conn
+         (%e_rl & #name & client & #server & not_ended &
+          #beginning & ending & status)".
+iPoseProof (conn_state_session with "conn") as "#sess".
+iFrame "conn".
+iAssert (|==> (session_fail cs ∨
+           nown γI (dbCN (si_resp cs).@"status")
+                (client_view (ClientDisconnecting (si_key cs) beginning
+                                (n + beginning)))))%I
+  with "[status]" as ">status".
+{ iDestruct "status" as "[fail|status]"; first by eauto.
+  iRight.
+  iApply (nown_update with "status").
+  exact: client_disconnect_update. }
+iAssert (|={E}=> conn_done cs γI beginning (n + beginning))%I
+  with "[status]" as ">#done".
+{ iApply (escrowI with "status").
+  iApply conn_ended_switch. }
+iMod (gmeta_set _ _ (nroot.@"db".@"ending") (n + beginning) with "ending")
+  as "#ending" => //.
+iSplitL.
+{ iFrame. by eauto. }
+iIntros "!> !>". iExists n, cs, γI, (cs_name cs), beginning.
+rewrite -e_rl. by eauto 10.
+Qed.
+
+Definition conn_closed si γI ending :=
+  escrow (nroot.@"db")
+         (conn_not_ended si Init)
+         (session_fail si ∨
+             nown γI (dbCN (si_resp si).@"status")
+                  (client_view (BothDisconnected ending))).
+
+Definition ack_close_pred kS (m : term) : iProp := ∃ si γ_sR,
+  ⌜si_key si = kS⌝ ∗
+  session γ_sR si Resp ∗
+  (session_fail si ∨ ∃ γI γ_sI ending,
+     key_name (si_init si) γI ∗
+     session γ_sI si Init ∗
+     gmeta γ_sI (nroot.@"db".@"ending") ending ∗
+     conn_closed si γI ending).
+
+Lemma ack_close_predI cs n db E :
+  let m := TInt n in
+  ↑nroot.@"db" ⊆ E →
+  is_conn_state cs n -∗
+  server_connected cs n db -∗
+  session_fail cs ∗ public m ∨ close_pred (si_key cs) m ={E}▷=∗
+  is_conn_state cs n ∗
+  server_disconnected (si_init cs) (si_resp cs) db ∗
+  □ ack_close_pred (si_key cs) (TInt 0).
+Proof.
+iIntros "%m %sub conn server p_m".
+iPoseProof (conn_state_session with "conn") as "#sessR".
+iFrame "conn".
+iDestruct "server" as "(%e_rl & not_ended & #p_db & status)".
+iAssert (□ (▷ session_fail cs ={E}▷=∗
+              server_disconnected (si_init cs) (si_resp cs) db ∗
+              □ ack_close_pred (si_key cs) (TInt 0)))%I
+  as "#failure".
+{ iIntros "!> #fail !> !> !>". iSplit.
+  - iSplit => //. iLeft.
+    by iDestruct "fail" as "[fail|fail]"; [iLeft|iRight];
+    iApply public_at_public.
+  - iModIntro. iExists _, _. rewrite e_rl. by eauto. }
+iDestruct "status" as "[#fail|status]"; first by iApply "failure".
+iDestruct "p_m" as "[[#fail _] | p_m]"; first by iApply "failure".
+iDestruct "status" as
+  "(%γI & %γ_sI & %beginning & #name & #sessI & #server &
+    #beginning & status)".
+iDestruct "p_m" as
+  "(%n' & %si & %γI' & %γ_sI' & %beginning' & %e_m & %e_kS &
+    #name' & #sessI' & #beginning' & #ending & #done)".
+iPoseProof (session_agree_name with "sessI' sessI") as
+  "[#fail | [-> ->]]" => //; first by iApply "failure".
+iClear "sessI'".
+iPoseProof (key_name_agree with "name name'") as "{name'} <-".
+iPoseProof (gmeta_agree with "beginning beginning'") as "{beginning'} <-".
+case: e_m => e_n. have {e_n} <- : n = n' by lia.
+iMod (escrowE with "done not_ended") as "[#fail|statusI]" => //;
+  first by iApply "failure".
+iIntros "!> !>".
+iMod (nown_update_2 with "statusI status") as "status".
+{ apply: server_disconnect_update. }
+iDestruct "status" as "[statusI status]".
+iAssert (|={E}=> conn_closed cs γI (n + beginning))%I
+  with "[statusI]" as ">#closed".
+{ iApply (escrowI with "[statusI]").
+  - by eauto.
+  - iApply conn_ended_switch. }
+iModIntro. iSplit.
+- iSplit => //. iRight. iRight. iExists _, _. iFrame. by eauto.
+- iModIntro. iExists cs, (cs_name cs). rewrite e_rl. do 2!iSplit => //.
+  iRight. iExists _, _, _. by eauto.
+Qed.
+
+Lemma ack_close_predE cs m γI n beginning E :
+  ↑nroot.@"db" ⊆ E →
+  is_conn_state cs n -∗
+  client_disconnecting_int cs γI n beginning -∗
+  session_fail cs ∗ public m ∨ ack_close_pred (si_key cs) m ={E}=∗
+  is_conn_state cs n ∗
+  ▷ client_disconnected_int (si_init cs) (si_resp cs) γI (n + beginning).
+Proof.
+iIntros "%sub conn (%e_rl & #name & client & #server & not_ended & #ending)".
+iIntros "p_m".
+iPoseProof (conn_state_session with "conn") as "#sessI".
+iFrame "conn".
+iDestruct "p_m" as "[[#fail _]|p_m]".
+{ iFrame. iSplitR => //. iSplitR => //. iLeft. iModIntro.
+  iDestruct "fail" as "[fail|fail]"; [iLeft|iRight];
+  by iApply public_at_public. }
+iDestruct "p_m" as "(%si & %γ_sR & %e_si & #sessR & p_m)" .
+iDestruct (session_agree with "sessR sessI") as "[fail|->]" => //.
+{ iFrame. do !iSplitR => //. iLeft. iModIntro.
+  iDestruct "fail" as "[fail|fail]"; [iLeft|iRight];
+  by iApply public_at_public. }
+iDestruct "p_m" as "[fail|p_m]".
+{ iFrame. do !iSplitR => //. iLeft. iModIntro.
+  iDestruct "fail" as "[fail|fail]"; [iLeft|iRight];
+  by iApply public_at_public. }
+iDestruct "p_m"
+  as "(%γI' & %γ_sI & %ending & #name' & #sessI' & #ending' & #closed)".
+rewrite e_rl.
+iDestruct (session_agree_name with "sessI sessI'") as "[fail|[_ <-]]" => //.
+{ iFrame. do !iSplitR => //. iLeft. iModIntro.
+  iDestruct "fail" as "[fail|fail]"; [iLeft|iRight];
+  by iApply public_at_public. }
+iPoseProof (gmeta_agree with "ending' ending") as "{ending'} ->".
+iPoseProof (key_name_agree with "name' name") as "{name' sessI'} ->".
+iMod (escrowE with "closed not_ended") as "[fail|status]" => //.
+{ iFrame. do !iSplitR => //. iLeft. iModIntro.
+  iDestruct "fail" as "[fail|fail]"; [iLeft|iRight];
+  by iApply public_at_public. }
+iFrame. by eauto.
+Qed.
+
+Definition server_handler_inv cs n ldb db : iProp :=
+  server_connected cs n db ∗
+  SAList.is_alist ldb (repr <$> db).
+
+Definition server_handler_post cs ldb v : iProp := ∃ n db,
+  ⌜v = #true⌝ ∗
+  is_conn_state cs n ∗
+  server_connected cs n db ∗
+  SAList.is_alist ldb (repr <$> db) ∨
+  ⌜v = #false⌝ ∗
+  is_conn_state cs n ∗
+  server_disconnected (si_init cs) (si_resp cs) db ∗
+  SAList.is_alist ldb (repr <$> db).
+
 Definition store_ctx : iProp :=
   enc_pred (N.@"init") init_pred ∗
+  enc_pred (N.@"ack_init") ack_init_pred ∗
   enc_pred (N.@"store") store_pred ∗
   enc_pred (N.@"ack_store") ack_store_pred ∗
   enc_pred (N.@"load") load_pred ∗
   enc_pred (N.@"ack_load") ack_load_pred ∗
   enc_pred (N.@"create") create_pred ∗
   enc_pred (N.@"ack_create") ack_create_pred ∗
+  enc_pred (N.@"close") close_pred ∗
+  enc_pred (N.@"ack_close") ack_close_pred ∗
   dh_auth_ctx (N.@"auth").
 
 Lemma store_ctx_alloc E :
@@ -143,99 +1405,85 @@ iIntros "%sub token".
 rewrite (enc_pred_token_difference (↑N)) => //.
 iDestruct "token" as "[token ?]". iFrame.
 iMod (enc_pred_set (N.@"init") init_pred with "token")
-  as "[#init token]"; try solve_ndisj.
+  as "[init token]"; try solve_ndisj.
+iFrame.
+iMod (enc_pred_set (N.@"ack_init") ack_init_pred with "token")
+  as "[ack_init token]"; try solve_ndisj.
+iFrame.
 iMod (enc_pred_set (N.@"store") store_pred with "token")
-  as "[#store token]"; try solve_ndisj.
+  as "[store token]"; try solve_ndisj.
+iFrame.
 iMod (enc_pred_set (N.@"ack_store") ack_store_pred with "token")
-  as "[#ack_store token]"; try solve_ndisj.
+  as "[ack_store token]"; try solve_ndisj.
+iFrame.
 iMod (enc_pred_set (N.@"load") load_pred with "token")
-  as "[#load token]"; try solve_ndisj.
+  as "[load token]"; try solve_ndisj.
+iFrame.
 iMod (enc_pred_set (N.@"ack_load") ack_load_pred with "token")
-  as "[#ack_load token]"; try solve_ndisj.
+  as "[ack_load token]"; try solve_ndisj.
+iFrame.
 iMod (enc_pred_set (N.@"create") create_pred with "token")
-  as "[#create token]"; try solve_ndisj.
+  as "[create token]"; try solve_ndisj.
+iFrame.
 iMod (enc_pred_set (N.@"ack_create") ack_create_pred with "token")
-  as "[#ack_create token]"; try solve_ndisj.
+  as "[ack_create token]"; try solve_ndisj.
+iFrame.
+iMod (enc_pred_set (N.@"close") close_pred with "token")
+  as "[close token]"; try solve_ndisj.
+iFrame.
+iMod (enc_pred_set (N.@"ack_close") ack_close_pred with "token")
+  as "[ack_close token]"; try solve_ndisj.
+iFrame.
 iMod (dh_auth_ctx_alloc (N.@"auth") with "token")
   as "#dh_auth"; try solve_ndisj.
-iModIntro. do !iSplit => //.
 Qed.
 
-Lemma initE si γ t :
-  store_ctx -∗
-  session γ si Resp -∗
-  □ (∀ kt, public (TKey kt (si_key si)) ↔ ▷ session_fail si) -∗
-  public (TEnc (si_key si) (Spec.tag (N.@"init") t)) -∗
-  ▷ (session_fail si ∨ ∃ γ, session γ si Init ∗ DB.server_view γ 0 ∅).
-Proof.
-iIntros "(#initP & _) #sessR #kS #p_t".
-iDestruct (public_TEncE with "[//] [//]") as "[[p_kS ?]|#tP]".
-{ iPoseProof ("kS" with "p_kS") as "comp".
-  iIntros "!>". by iLeft. }
-iDestruct "tP" as "(#init & _ & _)".
-iModIntro.
-iDestruct "init" as "(%si' & %γ' & %e_kS & sessI & #view)".
-iPoseProof (session_agree with "sessI sessR") as "[fail|->]"; by eauto.
-Qed.
+Ltac solve_ctx :=
+  iIntros "ctx"; repeat (
+    try solve [iApply "ctx"];
+    iDestruct "ctx" as "[H ctx]";
+    first [iApply "H" | iClear "H"]
+  ).
 
-Lemma store_predE si γ n t1 t2 :
-  store_ctx -∗
-  session γ si Resp -∗
-  □ (∀ kt, public (TKey kt (si_key si)) ↔ ▷ session_fail si) -∗
-  □ (session_fail si ∨ ∃ γ, session γ si Init) -∗
-  public (TEnc (si_key si) (Spec.tag (N.@"store")
-                              (Spec.of_list [TInt n; t1; t2]))) -∗
-  ▷ (public t1 ∗ public t2 ∗
-     (session_fail si ∨ ∃ γ, session γ si Init ∗ DB.update_at γ n t1 t2)).
-Proof.
-iIntros "#(_ & #storeP & _) #sessR #key #sessI #p_m".
-iPoseProof (public_TEncE with "p_m [//]") as "{p_m} p_m".
-rewrite public_of_list /=. iDestruct "p_m" as "[p_m|p_m]".
-- iDestruct "p_m" as "(p_k & p_m & ? & ? & ?)".
-  do 2!iSplit => //.
-  iPoseProof ("key" with "p_k") as "?".
-  by iLeft.
-- iModIntro.
-  iDestruct "p_m" as "(#(%n' & %t1' & %t2' & %si' & %γ' & mP) & _ & _)".
-  iDestruct "mP" as "(%e & %e_key & sessI' & p_t1 & p_t2 & update)".
-  case/Spec.of_list_inj: e => en <- <-.
-  have -> : n' = n by lia.
-  do 2!iSplitL => //.
-  iDestruct "sessI" as "[fail|(% & sessI)]"; first by iLeft.
-  iDestruct (session_agree_name with "sessI' sessI") as "[fail|(-> & <-)]"
-     => //; eauto.
-Qed.
+Lemma store_ctx_init : store_ctx -∗ enc_pred (N.@"init") init_pred.
+Proof. solve_ctx. Qed.
 
-Lemma ack_loadE si γ n t1 t2 t2' :
-  store_ctx -∗
-  session γ si Init -∗
-  □ (∀ kt, public (TKey kt (si_key si)) ↔ ▷ session_fail si) -∗
-  DB.client_view γ n -∗
-  DB.mapsto γ t1 t2 -∗
-  public (TEnc (si_key si) (Spec.tag (N.@"ack_load")
-         (Spec.of_list [TInt n; t1; t2']))) -∗
-  ▷ (public t2' ∗ (session_fail si ∨ ⌜t2' = t2⌝)).
-Proof.
-iIntros "#(_ & _ & _ & _ & ? & _) #sessI #key client mapsto #pub".
-iDestruct (public_TEncE with "pub [//]") as "{pub} [pub|pub]".
-- iDestruct "pub" as "[pub_k pub_t2]".
-  rewrite public_of_list /=.
-  iDestruct "pub_t2" as "(_ & _ & pub_t2 & _)".
-  iSplit => //.
-  iPoseProof ("key" with "pub_k") as "?".
-  by iLeft.
-- iDestruct "pub" as "(#pub & _ & _)". iModIntro.
-  iDestruct "pub" as "(%n' & %t1' & %t2'' & %si' & %γ' &
-                       %e & %e_kS & ? & #sessR & stored)".
-  case/Spec.of_list_inj: e => en <- <-.
-  have <- : n = n' by lia.
-  iSplit => //.
-  iPoseProof (session_agree with "sessR sessI") as "[fail|->]"; eauto.
-  iDestruct "stored" as "[fail|(%γ'' & sessI' & stored)]"; eauto.
-  iDestruct (session_agree_name with "sessI' sessI") as "[fail|(_ & ->)]"; eauto.
-  iPoseProof (DB.load_client with "client mapsto stored") as "->".
-  eauto.
-Qed.
+Lemma store_ctx_ack_init : store_ctx -∗ enc_pred (N.@"ack_init") ack_init_pred.
+Proof. solve_ctx. Qed.
+
+Lemma store_ctx_store : store_ctx -∗ enc_pred (N.@"store") store_pred.
+Proof. solve_ctx. Qed.
+
+Lemma store_ctx_ack_store :
+  store_ctx -∗ enc_pred (N.@"ack_store") ack_store_pred.
+Proof. solve_ctx. Qed.
+
+Lemma store_ctx_load :
+  store_ctx -∗ enc_pred (N.@"load") load_pred.
+Proof. solve_ctx. Qed.
+
+Lemma store_ctx_ack_load :
+  store_ctx -∗ enc_pred (N.@"ack_load") ack_load_pred.
+Proof. solve_ctx. Qed.
+
+Lemma store_ctx_create :
+  store_ctx -∗ enc_pred (N.@"create") create_pred.
+Proof. solve_ctx. Qed.
+
+Lemma store_ctx_ack_create :
+  store_ctx -∗ enc_pred (N.@"ack_create") ack_create_pred.
+Proof. solve_ctx. Qed.
+
+Lemma store_ctx_close :
+  store_ctx -∗ enc_pred (N.@"close") close_pred.
+Proof. solve_ctx. Qed.
+
+Lemma store_ctx_ack_close :
+  store_ctx -∗ enc_pred (N.@"ack_close") ack_close_pred.
+Proof. solve_ctx. Qed.
+
+Lemma store_ctx_dh_auth_ctx : store_ctx -∗ dh_auth_ctx (N.@"auth").
+Proof. solve_ctx. Qed.
 
 End Defs.
 
