store/client_proofs.v
@@ -1,2 +1,2 @@
 From cryptis.store.client_proofs
-  Require Export common store load create connect.
+  Require Export store load create connect close.
