store/client_proofs/close.v
@@ -1,0 +1,65 @@
+From stdpp Require Import base gmap.
+From mathcomp Require Import ssreflect.
+From stdpp Require Import namespaces.
+From iris.algebra Require Import agree auth csum gset gmap excl frac.
+From iris.algebra Require Import max_prefix_list.
+From iris.heap_lang Require Import notation proofmode.
+From cryptis Require Import lib version term gmeta nown cryptis.
+From cryptis Require Import primitives tactics role dh_auth.
+From cryptis.store Require Import impl shared db connection_proofs.
+
+Set Implicit Arguments.
+Unset Strict Implicit.
+Unset Printing Implicit Defensive.
+
+Section Verif.
+
+Context `{!cryptisGS Σ, !heapGS Σ, !sessionGS Σ, !storeGS Σ}.
+Notation iProp := (iProp Σ).
+
+Context `{!storeG Σ}.
+
+Implicit Types (cs : conn_state).
+Implicit Types kI kR kS t : term.
+Implicit Types n : nat.
+Implicit Types γ : gname.
+Implicit Types v : val.
+
+Variable N : namespace.
+
+Lemma wp_client_close E c kI kR cs :
+  ↑cryptisN ⊆ E →
+  ↑nroot.@"db" ⊆ E →
+  channel c -∗
+  store_ctx N -∗
+  {{{ client_connected kI kR cs }}}
+    Client.close N c (repr cs) @ E
+  {{{ RET #();
+      client_disconnected kI kR }}}.
+Proof.
+iIntros "% % #chan_c (_ & _ & _ & _ & _ & _ & _ & _ & #close & #ack & _)".
+iIntros "!> %Φ client post".
+iDestruct "client" as "(%γI & %n & %beginning & <- & <- & conn & client)".
+wp_lam; wp_pures.
+wp_bind (Connection.timestamp _).
+iApply (wp_connection_timestamp with "conn").
+iIntros "!> conn". wp_pures.
+wp_bind (tint _). iApply wp_tint. wp_pures.
+iMod (close_predI with "conn client") as "(conn & client & #p_m1)" => //.
+wp_bind (Connection.send _ _ _ _).
+iApply (wp_connection_send with "[//] close [] [//] conn") => //.
+{ by rewrite public_TInt. }
+iIntros "!> conn". wp_pures.
+iCombine "client post" as "I". iRevert "conn I".
+iApply wp_connection_recv => //.
+iIntros "!> %m conn (client & post) #m_m #inv'".
+iMod (ack_close_predE with "conn client inv'") as "(conn & client)" => //.
+wp_pures. wp_bind (Connection.close _ _).
+iApply (wp_connection_close with "conn"). iIntros "!> _".
+wp_pures.
+iRight. iModIntro. iExists _. iSplit; eauto.
+iApply "post".
+iExists _, _. by eauto.
+Qed.
+
+End Verif.
