store/client_proofs/create.v
@@ -4,10 +4,9 @@ From stdpp Require Import namespaces.
 From iris.algebra Require Import agree auth csum gset gmap excl frac.
 From iris.algebra Require Import max_prefix_list.
 From iris.heap_lang Require Import notation proofmode.
-From cryptis Require Import lib version term cryptis primitives tactics.
-From cryptis Require Import role dh_auth.
-From cryptis.store Require Import impl shared db.
-From cryptis.store.client_proofs Require Import common.
+From cryptis Require Import lib version term gmeta nown cryptis.
+From cryptis Require Import primitives tactics role dh_auth.
+From cryptis.store Require Import impl shared db connection_proofs.
 
 Set Implicit Arguments.
 Unset Strict Implicit.
@@ -20,7 +19,7 @@ Notation iProp := (iProp Σ).
 
 Context `{!storeG Σ}.
 
-Implicit Types (cs : cst).
+Implicit Types (cs : conn_state).
 Implicit Types kI kR kS t : term.
 Implicit Types n : nat.
 Implicit Types γ : gname.
@@ -28,47 +27,42 @@ Implicit Types v : val.
 
 Variable N : namespace.
 
-Lemma wp_client_create E c cs t1 t2 :
+Lemma wp_client_create E c kI kR cs t1 t2 :
   ↑cryptisN ⊆ E →
   channel c -∗
   store_ctx N -∗
   public t1 -∗
   public t2 -∗
-  {{{ client cs ∗ rem_free_at cs {[t1]} }}}
+  {{{ client_connected kI kR cs ∗
+      rem_free_at kI kR {[t1]} }}}
     Client.create N c (repr cs) t1 t2 @ E
   {{{ (b : bool), RET #b;
-      client cs ∗
-      rem_mapsto cs t1 t2 }}}.
+      client_connected kI kR cs ∗
+      rem_mapsto kI kR t1 t2 }}}.
 Proof.
-iIntros "% #chan_c (_ & _ & _ & _ & _ & #? & #? & _)
-         #p_t1 #p_t2' !> %Φ [client free] post".
-iDestruct "client" as "(%n & #handshake & #key & #minted & ts & client)".
+iIntros "% #chan_c (_ & _ & _ & _ & _ & _ & #create & #ack & _) #p_t1 #p_t2".
+iIntros "!> %Φ [client free] post".
+iDestruct "client" as "(%γI & %n & %beginning & <- & <- & conn & client)".
 rewrite /Client.create. wp_pures.
-wp_bind (Client.get_timestamp _).
-iApply (wp_client_get_timestamp with "ts").
-iIntros "!> ts". wp_pures.
-wp_bind (Client.get_session_key _).
-iApply wp_client_get_session_key => //.
-iIntros "!> _". wp_pures.
+iMod (@rem_mapsto_alloc _ _ _ _ _ _ t1 t2 with "conn client free")
+  as "(conn & client & mapsto & _ & #created)".
+{ by rewrite elem_of_singleton. }
+wp_bind (Connection.timestamp _).
+iApply (wp_connection_timestamp with "conn").
+iIntros "!> conn". wp_pures.
+wp_bind (Connection.tick _).
+iApply (wp_connection_tick with "conn"). iIntros "!> conn".
+iDestruct (create_predI with "conn client p_t1 p_t2 created")
+  as "(conn & client & #p_m1)".
 wp_list. wp_bind (tint _). iApply wp_tint. wp_list. wp_term_of_list. wp_pures.
-wp_tsenc. wp_pures.
-iMod (DB.create_client t1 t2 with "client free")
-  as "(#create & client & up)".
-wp_bind (send _ _). iApply wp_send => //.
-{ iApply public_TEncIS => //.
-  - by rewrite minted_TKey.
-  - iModIntro. iExists n, t1, t2, cs, (cst_name cs).
-    by eauto 8.
-  - rewrite minted_of_list /= minted_TInt.
-    rewrite -[minted t1]public_minted -[minted t2]public_minted.
-    by eauto.
-  - iIntros "!> !> _".
-    rewrite public_of_list /= public_TInt. by eauto. }
-wp_pures.
-iCombine "post ts client up" as "I". iRevert "I".
-iApply wp_sess_recv => //.
-iIntros "!> %m (post & ts & client & up) #p_m". wp_pures.
-wp_list_of_term m; wp_pures; last by iLeft; iFrame.
+wp_bind (Connection.send _ _ _ _).
+iApply (wp_connection_send with "[//] create [] [//] conn") => //.
+{ by rewrite public_of_list /= public_TInt; eauto. }
+iIntros "!> conn". wp_pures.
+iCombine "client mapsto post" as "I". iRevert "conn I".
+iApply wp_connection_recv => //.
+iIntros "!> %m conn (client & mapsto & post) #m_m #inv'".
+wp_pures. wp_list_of_term m; wp_pures; last by iLeft; iFrame.
 wp_list_match => [ts' k' v' b -> {m}|_] /=; wp_pures; last by iLeft; iFrame.
 wp_bind (tint _). iApply wp_tint.
 wp_eq_term e; wp_pures; last by iLeft; iFrame.
@@ -77,13 +71,10 @@ wp_eq_term e; wp_pures; last by iLeft; iFrame.
 subst k'.
 wp_eq_term e; wp_pures; last by iLeft; iFrame.
 subst v'.
-wp_bind (Client.incr_timestamp _).
-iApply (wp_client_incr_timestamp with "ts").
-iIntros "!> ts".
-wp_pures. wp_bind (tint _). iApply wp_tint.
+wp_bind (tint _). iApply wp_tint.
 wp_bind (eq_term _ _). iApply wp_eq_term. wp_pures.
 iRight. iModIntro. iExists _. iSplit => //. iApply "post".
-iFrame. iExists (S n). iFrame. do !iSplit => //.
+iFrame. iExists _, _, _. iFrame. do !iSplit => //.
 Qed.
 
 End Verif.
