store/client_proofs/store.v
@@ -6,8 +6,7 @@ From iris.algebra Require Import max_prefix_list.
 From iris.heap_lang Require Import notation proofmode.
 From cryptis Require Import lib version term cryptis primitives tactics.
 From cryptis Require Import role dh_auth.
-From cryptis.store Require Import impl shared db.
-From cryptis.store.client_proofs Require Import common.
+From cryptis.store Require Import impl shared db connection_proofs.
 
 Set Implicit Arguments.
 Unset Strict Implicit.
@@ -20,7 +19,7 @@ Notation iProp := (iProp Σ).
 
 Context `{!storeG Σ}.
 
-Implicit Types (cs : cst).
+Implicit Types (cs : conn_state).
 Implicit Types kI kR kS t : term.
 Implicit Types n : nat.
 Implicit Types γ : gname.
@@ -28,75 +27,67 @@ Implicit Types v : val.
 
 Variable N : namespace.
 
-Lemma wp_client_send_store E c cs t1 t2 t2' :
+Lemma wp_client_send_store E c kI kR cs t1 t2 t2' :
   ↑cryptisN ⊆ E →
   channel c -∗
   store_ctx N -∗
   public t1 -∗
-  public t2' -∗ (* FIXME: t1 and t2' do not have to be public already *)
-  {{{ client cs ∗ rem_mapsto cs t1 t2 }}}
+  public t2' -∗ (* FIXME: t1 and t2' shouldn't have to be public already *)
+  {{{ client_connected kI kR cs ∗ rem_mapsto kI kR t1 t2 }}}
     Client.send_store N c (repr cs) t1 t2' @ E
-  {{{ RET #(); client cs ∗ rem_mapsto cs t1 t2' }}}.
+  {{{ RET #(); client_connected kI kR cs ∗ rem_mapsto kI kR t1 t2' }}}.
 Proof.
-rewrite /Client.send_store /rem_mapsto.
-iIntros "% #chan_c (_ & #? & _) #p_t1 #p_t2' !> %Φ [client mapsto] post".
-iDestruct "client" as "(%n & #handshake & #key & #minted & ts & client)".
-iMod (DB.update_client t2' with "client mapsto") as "(client & #update & mapsto)".
-wp_pures. wp_bind (Client.get_timestamp _).
-iApply (wp_client_get_timestamp with "ts"); iIntros "!> ts".
-wp_pures. wp_bind (Client.incr_timestamp _).
-iApply (wp_client_incr_timestamp with "ts"). iIntros "!> ts".
-wp_pures. wp_bind (Client.get_session_key _).
-iApply (wp_client_get_session_key with "[//]"); iIntros "!> _".
+iIntros "% #chan_c (_ & _ & #? & _) #p_t1 #p_t2' !> %Φ [client mapsto] post".
+iDestruct "client" as "(%γI & %n & %beginning & <- & <- & conn & client)".
+iMod (rem_mapsto_update t2' with "conn client mapsto")
+  as "(client & conn & mapsto & #update)".
+wp_lam. wp_pures. wp_bind (Connection.timestamp _).
+iApply (wp_connection_timestamp with "conn"); iIntros "!> conn".
+wp_pures. wp_bind (Connection.tick _).
+iApply (wp_connection_tick with "conn"). iIntros "!> conn".
+iPoseProof (store_predI with "conn client p_t1 p_t2' update")
+  as "(conn & client & #?)".
 wp_pures. wp_list. wp_bind (tint _). iApply wp_tint. wp_list.
-wp_term_of_list. wp_tsenc. wp_pures.
-iPoseProof ("post" with "[client ts mapsto]") as "post".
-{ iFrame. iExists (S n). iFrame. by eauto. }
-iApply (wp_send with "[//] [#]") => //. iClear "post".
-iModIntro. iApply public_TEncIS => //.
-- by rewrite minted_TKey.
-- iModIntro. iExists n, t1, t2', cs, (cst_name cs).
-  do 5?iSplit => //.
-- rewrite minted_of_list /= minted_TInt; do ![iSplit => //];
-  by iApply public_minted.
-- iModIntro. iIntros "_". rewrite public_of_list /= public_TInt. iSplit => //.
-  by eauto.
+wp_term_of_list. wp_pures.
+iApply (wp_connection_send with "[//] [//] [] [#] conn") => //.
+- rewrite public_of_list /= public_TInt. by eauto.
+iIntros "!> conn".
+iApply ("post" with "[conn client mapsto]").
+iFrame. iExists _, _, _. by iFrame.
 Qed.
 
-Lemma wp_client_ack_store E c cs :
+Lemma wp_client_ack_store E c kI kR cs :
   ↑cryptisN ⊆ E →
   channel c -∗
   store_ctx N -∗
-  {{{ client cs }}}
+  {{{ client_connected kI kR cs }}}
     Client.ack_store N c (repr cs) @ E
-  {{{ RET #(); client cs }}}.
+  {{{ RET #(); client_connected kI kR cs }}}.
 Proof.
-iIntros "% #chan_c (_ & _ & #? & _) !> %Φ client post".
+iIntros "% #chan_c (_ & _ & _ & #? & _) !> %Φ client post".
+iDestruct "client" as "(%γI & %n & %beginning & <- & <- & conn & client)".
 rewrite /Client.ack_store. wp_pures.
-iDestruct "client" as "(%n & #handshake & #key & #minted & ts & client)".
-wp_bind (Client.get_timestamp _).
-iApply (wp_client_get_timestamp with "ts"). iIntros "!> ts". wp_pures.
-wp_bind (Client.get_session_key _).
-iApply (wp_client_get_session_key with "[//]") => //.
-iIntros "!> _". wp_pures.
-iCombine "client post ts" as "I". iRevert "I".
-iApply wp_sess_recv => //. iIntros "!> %m (client & post & ts) _".
+wp_bind (Connection.timestamp _).
+iApply (wp_connection_timestamp with "conn"). iIntros "!> conn".
+wp_pures.
+iCombine "client post" as "I". iRevert "conn I".
+iApply wp_connection_recv => //.
+iIntros "!> %m conn (client & post) #m_m _".
 wp_pures. wp_bind (tint _). iApply wp_tint.
-wp_eq_term e; wp_pures; iModIntro; last first.
-  iLeft. by iFrame.
-iRight. iExists _; iSplit => //. iApply "post".
-iExists n. by iFrame; eauto.
+wp_eq_term e; wp_pures; last by iLeft; iFrame.
+iRight. iModIntro. iExists _. iSplit => //.
+iApply "post". by iExists _, _, _; iFrame.
 Qed.
 
-Lemma wp_client_store E c cs t1 t2 t2' :
+Lemma wp_client_store E c kI kR cs t1 t2 t2' :
   ↑cryptisN ⊆ E →
   channel c -∗
   store_ctx N -∗
   public t1 -∗
   public t2' -∗
-  {{{ client cs ∗ rem_mapsto cs t1 t2 }}}
+  {{{ client_connected kI kR cs ∗ rem_mapsto kI kR t1 t2 }}}
     Client.store N c (repr cs) t1 t2' @ E
-  {{{ RET #(); client cs ∗ rem_mapsto cs t1 t2' }}}.
+  {{{ RET #(); client_connected kI kR cs ∗ rem_mapsto kI kR t1 t2' }}}.
 Proof.
 iIntros "% #chan_c #ctx #p_t1 #p_t2 !> %Φ [client mapsto] post".
 rewrite /Client.store.
