store/connection_proofs.v
@@ -1,0 +1,367 @@
+From stdpp Require Import base gmap.
+From mathcomp Require Import ssreflect.
+From stdpp Require Import namespaces.
+From iris.algebra Require Import agree auth csum gset gmap excl frac.
+From iris.algebra Require Import max_prefix_list.
+From iris.heap_lang Require Import notation proofmode.
+From cryptis Require Import lib version term gmeta cryptis primitives tactics.
+From cryptis Require Import role dh_auth.
+From cryptis.store Require Import impl shared.
+
+Set Implicit Arguments.
+Unset Strict Implicit.
+Unset Printing Implicit Defensive.
+
+Section Verif.
+
+Context `{!cryptisGS Σ, !heapGS Σ}.
+Notation iProp := (iProp Σ).
+
+Implicit Types (cs : conn_state).
+Implicit Types kI kR kS t : term.
+Implicit Types n : nat.
+Implicit Types γ : gname.
+Implicit Types v : val.
+
+Lemma wp_connection_connect N E c kI kR dq n T :
+  ↑cryptisN ⊆ E →
+  channel c -∗
+  cryptis_ctx -∗
+  dh_auth_ctx (N.@"auth") -∗
+  public (TKey Dec kI) -∗
+  public (TKey Dec kR) -∗
+  {{{ ●H{dq|n} T }}}
+    Connection.connect N c (TKey Enc kI) (TKey Dec kI) (TKey Dec kR)
+    @ E
+  {{{ cs, RET (repr cs);
+    ●H{dq|n} T ∗
+    is_conn_state cs 0 ∗
+    ⌜si_init cs = kI⌝ ∗
+    ⌜si_resp cs = kR⌝ ∗
+    ⌜si_time cs = n⌝ ∗
+    ⌜si_hon cs = T⌝ ∗
+    ⌜cs_role cs = Init⌝ ∗
+    gmeta_token (cs_name cs) (⊤ ∖ ↑nroot.@"dh_auth") }}}.
+Proof.
+iIntros "% #? #? #? #? #? % !> hon post".
+wp_lam. wp_pures.
+iCombine "hon post" as "I". iRevert "I".
+iApply wp_do_until. iIntros "!> [hon post]".
+wp_pures. wp_bind (initiator _ _ _ _ _).
+iApply (wp_initiator with "[//] [//] [//] [] [] [hon]") => //.
+iIntros "!> %res (hon & resP)".
+case: res=> [kS|] /=; wp_pures; last by iLeft; iFrame; eauto.
+wp_alloc ts as "ts". set  si := SessInfo _ _ _ _ _. wp_pures.
+iDestruct "resP" as "(%γ & #m_kS & #sess & token & #p_kS)".
+iRight. iModIntro. iExists _.  iSplit => //.
+iApply ("post" $! (ConnState si ts γ Init)). iFrame => /=.
+eauto.
+Qed.
+
+Lemma wp_connection_listen N E c kR dq n T :
+  ↑cryptisN ⊆ E →
+  channel c -∗
+  cryptis_ctx -∗
+  dh_auth_ctx (N.@"auth") -∗
+  public (TKey Dec kR) -∗
+  {{{ ●H{dq|n} T }}}
+    Connection.listen N c (TKey Enc kR) (TKey Dec kR)
+    @ E
+  {{{ cs, RET (TKey Dec (si_init cs), repr cs)%V;
+    ●H{dq|n} T ∗
+    is_conn_state cs 0 ∗
+    ⌜si_resp cs = kR⌝ ∗
+    ⌜si_time cs = n⌝ ∗
+    ⌜si_hon cs = T⌝ ∗
+    ⌜cs_role cs = Resp⌝ ∗
+    gmeta_token (cs_name cs) (⊤ ∖ ↑nroot.@"dh_auth") }}}.
+Proof.
+iIntros "% #? #? #? #? % !> hon post".
+wp_lam. wp_pures.
+iCombine "hon post" as "I". iRevert "I".
+iApply wp_do_until. iIntros "!> [hon post]".
+wp_pures. wp_bind (responder _ _ _ _).
+iApply (wp_responder with "[//] [//] [] [] [hon]") => //.
+iIntros "!> %res (hon & resP)".
+case: res=> [[vkI kS]|] /=; wp_pures; last by iLeft; iFrame; eauto.
+wp_alloc ts as "ts".
+iDestruct "resP" as "(%kI & %γ & -> & #p_vkI & #m_kS & #sess & token & #p_kS)".
+set  si := SessInfo _ _ _ _ _. wp_pures.
+iRight. iModIntro. iExists _.  iSplit => //.
+iApply ("post" $! (ConnState si ts γ Resp)). iFrame => /=.
+eauto.
+Qed.
+
+Lemma wp_connection_timestamp E cs (n : nat) :
+  {{{ is_conn_state cs n }}}
+    Connection.timestamp (repr cs) @ E
+  {{{ RET #n; is_conn_state cs n }}}.
+Proof.
+rewrite /Connection.timestamp.
+iIntros "%Φ (Hn & #sess & #? & #key) post".
+wp_pures. wp_load. iApply "post". iModIntro. iFrame. by eauto.
+Qed.
+
+Lemma wp_connection_tick E cs (n : nat) :
+  {{{ is_conn_state cs n }}}
+    Connection.tick (repr cs) @ E
+  {{{ RET #(); is_conn_state cs (S n) }}}.
+Proof.
+iIntros "%Ψ (Hn & #seas & #? & #key) post".
+rewrite /Connection.tick; wp_pures; wp_load; wp_store.
+iApply "post".
+rewrite (_ : (n + 1)%Z = (S n)%nat :> Z); last by lia.
+iFrame; eauto.
+Qed.
+
+Lemma wp_connection_session_key E cs n :
+  {{{ is_conn_state cs n }}}
+    Connection.session_key (repr cs) @ E
+  {{{ RET (repr (Spec.mkskey (si_key cs)));
+      is_conn_state cs n ∗
+      session (cs_name cs) cs (cs_role cs) ∗
+      minted (si_key cs) ∗
+      □ (∀ kt, public (TKey kt (si_key cs)) ↔ ▷ session_fail cs) }}}.
+Proof.
+rewrite /Connection.session_key.
+iIntros "%Φ (? & #? & #? & #?) post". wp_pures. iApply "post".
+iModIntro. iFrame. iSplit => //; eauto.
+Qed.
+
+Lemma wp_connection_send N E c cs n m φ :
+  ↑cryptisN ⊆ E →
+  channel c -∗
+  enc_pred N φ -∗
+  public m -∗
+  □ φ (si_key cs) m -∗
+  {{{ is_conn_state cs n }}}
+    Connection.send N c (repr cs) m @ E
+  {{{ RET #(); is_conn_state cs n }}}.
+Proof.
+iIntros "%sub #chan #pred #public_m #inv !> %Φ conn post".
+wp_lam. wp_pures.
+wp_bind (Connection.session_key _).
+iApply (wp_connection_session_key with "conn").
+iIntros "!> (conn & #sess & #minted_k & #sec)". wp_pures.
+wp_bind (tsenc _ _ _). iApply wp_tsenc. wp_pures.
+iApply wp_send => //.
+{ iApply public_TEncIS => //.
+  - by rewrite minted_TKey.
+  - by iApply public_minted.
+  - by iIntros "!> !> _". }
+by iApply "post".
+Qed.
+
+Lemma wp_connection_select_body φ v (handlers : list val) (Φ : val → iProp) E :
+  ([∗ list] handler ∈ handlers,
+    (φ -∗ WP (handler : val) v @ E {{ v',
+           ⌜v' = NONEV⌝ ∗ φ ∨
+           ∃ r, ⌜v' = SOMEV r⌝ ∗ Φ r }}))%I -∗
+  φ -∗ WP Connection.select_body v (repr handlers) @ E {{ v',
+      ⌜v' = NONEV⌝ ∗ φ ∨
+      ∃ r, ⌜v' = SOMEV r⌝ ∗ Φ r }}.
+Proof.
+rewrite /= repr_list_unseal.
+iIntros "wp_handlers inv".
+iLöb as "IH" forall (handlers).
+wp_rec; case: handlers=> [|handler handlers]; wp_pures; first by eauto.
+rewrite /=. iDestruct "wp_handlers" as "[wp_handler wp_handlers]".
+iSpecialize ("wp_handler" with "inv").
+iSpecialize ("IH" with "wp_handlers").
+wp_bind (handler _); iApply (wp_wand with "wp_handler").
+iIntros "%v' [[-> inv] | (%r & -> & post)]"; wp_pures.
+- by iApply "IH".
+- iRight. iExists r. by iFrame.
+Qed.
+
+Lemma wp_connection_select_body' Φ φ v (handlers : list val) Ψ E :
+  ([∗ list] handler ∈ handlers,
+     (φ -∗ WP (handler : val) v @ E {{ v,
+       ⌜v = NONEV⌝ ∗ φ ∨
+       ∃ r, ⌜v = SOMEV r⌝ ∗ Φ r }}))%I -∗
+  (φ -∗ Ψ NONEV) -∗
+  (∀ r, Φ r -∗ Ψ (SOMEV r)) -∗
+  φ -∗
+  WP Connection.select_body v (repr handlers) @ E {{ Ψ }}.
+Proof.
+iIntros "wp post1 post2 inv".
+iApply (wp_wand with "[wp inv] [post1 post2]").
+- by iApply (wp_connection_select_body φ v handlers Φ with "[wp] inv").
+- iIntros "%res [[-> ?]|(%r & -> & ?)]".
+  + by iApply "post1".
+  + by iApply "post2".
+Qed.
+
+Lemma wp_connection_make_handler φ Φ k (handler : namespace * expr) E :
+  WP handler.2 @ E {{ f,
+    □ ∀ m : term,
+        public (TEnc k (Spec.tag handler.1 m)) -∗
+        φ -∗
+        WP (f : val) m @ E {{ v',
+            ⌜v' = NONEV⌝ ∗ φ ∨
+            ∃ r, ⌜v' = SOMEV r⌝ ∗ Φ r }}
+  }} -∗
+  WP Connection.make_handler handler @ E {{ f,
+    □ ∀ m : term,
+        public (TEnc k m) -∗
+        φ -∗
+        WP (f : val) m @ E {{ v',
+          ⌜v' = NONEV⌝ ∗ φ ∨
+          ∃ r, ⌜v' = SOMEV r⌝ ∗ Φ r }}
+  }}.
+Proof.
+case: handler => N handler /=; iIntros "wp".
+rewrite /Connection.make_handler. wp_pures.
+wp_bind handler. iApply (wp_wand with "wp").
+iIntros "%handler' #Hhandler'". wp_pures.
+iIntros "!> !> %m #p_m inv". wp_pures.
+wp_untag m; wp_pures.
+- by iApply "Hhandler'".
+- by iLeft; iFrame.
+Qed.
+
+Lemma wp_connection_make_handlers φ Φ k (handlers : list (namespace * expr)) E :
+  ([∗ list] handler ∈ handlers,
+      WP (handler.2 : expr) @ E {{ f, □ ∀ m : term,
+        public (TEnc k (Spec.tag handler.1 m)) -∗
+        φ -∗
+        WP (f : val) m @ E {{ v,
+            ⌜v = NONEV⌝ ∗ φ ∨
+            ∃ r, ⌜v = SOMEV r⌝ ∗ Φ r }} }})%I -∗
+  WP Connection.make_handlers handlers @ E {{ v',
+    ∃ handlers' : list val, ⌜v' = repr handlers'⌝ ∗
+      [∗ list] handler' ∈ handlers', □ ∀ m : term,
+        public (TEnc k m) -∗
+        φ -∗
+        WP (handler' : val) m @ E {{ v,
+          ⌜v = NONEV⌝ ∗ φ ∨
+          ∃ r, ⌜v = SOMEV r⌝ ∗ Φ r }}
+  }}.
+Proof.
+rewrite /= repr_list_unseal.
+elim: handlers=> [|[N handler] handlers IH] //=.
+  iIntros "_". wp_pures. iModIntro. iExists []. by rewrite /=.
+iIntros "[wp_handler wp_handlers]".
+wp_bind (Connection.make_handlers _).
+iPoseProof (IH with "wp_handlers") as "wp_handlers". clear IH.
+iApply (wp_wand with "wp_handlers [wp_handler]").
+iIntros "%v' (%handlers' & -> & #Hhandlers')".
+wp_bind (Connection.make_handler _).
+iApply (wp_wand with "[wp_handler] [Hhandlers']").
+{ iApply (wp_connection_make_handler _ _ _ (N, handler) with "wp_handler"). }
+iIntros "%f #wp_f". wp_lam; wp_pures.
+iExists (f :: handlers'). iSplitR => //=.
+iModIntro. iSplit => //.
+Qed.
+
+Definition handler_correct φ Φ cs handler n E : iProp :=
+  WP handler.2 @ E {{ f,
+    ∃ Ψ, enc_pred handler.1 Ψ ∗
+    □ ∀ m, minted m -∗
+           □ ▷ (session_fail cs ∗ public m ∨ Ψ (si_key cs) m) -∗
+           is_conn_state cs n -∗
+           φ -∗
+           WP (f : val) m @ E {{ v,
+             ⌜v = NONEV⌝ ∗ is_conn_state cs n ∗ φ ∨
+             ∃ r, ⌜v = SOMEV r⌝ ∗ Φ r }}
+  }}%I.
+
+Lemma wp_connection_select φ Φ (c : val) cs n (handlers : list (namespace * expr)) E :
+  ↑cryptisN ⊆ E →
+  channel c -∗
+  ([∗ list] handler ∈ handlers, handler_correct φ Φ cs handler n E) -∗
+  is_conn_state cs n -∗
+  φ -∗
+  WP Connection.select c (repr cs) handlers @ E {{ Φ }}.
+Proof.
+rewrite Connection.select_eq /Connection.select_def.
+iIntros "%sub #chan_c wps conn inv".
+wp_bind (Connection.make_handlers _).
+iApply (wp_wand with "[wps]").
+{ iApply (wp_connection_make_handlers
+            (is_conn_state cs n ∗ φ) Φ (si_key cs)
+           with "[wps]").
+  iApply (big_sepL_impl with "wps").
+  iIntros "!> % %handler _ wp".
+  iApply (wp_wand with "wp").
+  iIntros "%f #wp !> %m #p_m [conn inv]".
+  iDestruct "wp" as "(%Ψ & #enc & #wp)".
+  iAssert (minted m) as "#m_m".
+  { rewrite public_minted minted_TEnc minted_tag.
+    by iDestruct "p_m" as "[??]". }
+  iPoseProof (public_TEncE with "p_m enc") as "{p_m} p_m".
+  iAssert (□ ∀ kt, public (TKey kt (si_key cs)) ↔ ▷ session_fail cs)%I as "#p_kS".
+  { by iDestruct "conn" as "(_ & _ & _ & #?)". }
+  iApply ("wp" with "m_m [] conn inv").
+  iDestruct "p_m" as "[[fail p_m]|(#inv & ?)]".
+  - iSpecialize ("p_kS" with "fail"). by eauto.
+  - by eauto. }
+iIntros "% (%handlers' & -> & #Hhandlers')".
+wp_pures.
+wp_bind (Connection.session_key _).
+iApply (wp_connection_session_key with "conn").
+iIntros "!> (conn & #sess & #m_kS & #p_kS)".
+wp_bind (untuple _).
+iApply wp_untuple => /=.
+wp_pures. iCombine "conn inv" as "I". iRevert "I". iApply wp_do_until.
+iIntros "!> I". wp_pures. wp_bind (recv _). iApply wp_recv => //.
+iIntros "%m #p_m". wp_pures.
+wp_dec m; wp_pures; last by iLeft; iFrame.
+iApply (wp_connection_select_body' Φ with "[] [] [] I").
+- iApply (big_sepL_impl with "Hhandlers'").
+  iIntros "!> %k %handler _ #Hhandler inv" => //.
+  by iApply ("Hhandler" with "p_m inv").
+- iIntros "[??]". iLeft. by iFrame.
+- iIntros "%r Hr". iRight. iExists r. by eauto.
+Qed.
+
+Lemma wp_connection_recv N E c cs n (f : val) φ Φ Ψ :
+  ↑cryptisN ⊆ E →
+  channel c -∗
+  enc_pred N Φ -∗
+  □ (∀ m,
+      is_conn_state cs n -∗
+      φ -∗
+      minted m -∗
+      □ (session_fail cs ∗ public m ∨ Φ (si_key cs) m) -∗
+      WP f m @ E {{ v, ⌜v = NONEV⌝ ∗ is_conn_state cs n ∗ φ ∨
+                       ∃ v', ⌜v = SOMEV v'⌝ ∗ Ψ v' }}) -∗
+  is_conn_state cs n -∗ φ -∗ WP Connection.recv N c (repr cs) f @ E {{ Ψ }}.
+Proof.
+iIntros "%sub #chan #pred #post conn inv".
+wp_lam; wp_pures.
+wp_bind (Connection.session_key _).
+iApply (wp_connection_session_key with "conn").
+iIntros "!> (conn & #sess & #minted_kS & #p_kS)".
+wp_pures. iCombine "conn inv" as "I". iRevert "I".
+iApply wp_do_until.
+iIntros "!> (conn & inv)".
+wp_pure _ credit:"c".
+wp_pures. wp_bind (recv _). iApply wp_recv => //.
+iIntros "%m #p_m". wp_pures. wp_tsdec m; wp_pures; last by iLeft; iFrame.
+iAssert (▷ □ (session_fail cs ∗ public m ∨ Φ (si_key cs) m))%I
+  as "p_m'".
+{ iDestruct (public_TEncE with "[//] [//]") as "{p_m} [[fail p_m]|p_m]".
+  - iPoseProof ("p_kS" with "fail") as "{fail} fail".
+    iModIntro. by eauto.
+  - iDestruct "p_m" as "[p_m ?]".
+    iModIntro. iModIntro. eauto. }
+iMod (lc_fupd_elim_later with "c p_m'") as "{p_m'} #p_m'".
+iApply ("post" with "conn inv").
+{ rewrite public_minted minted_TEnc minted_tag.
+  by iDestruct "p_m" as "[??]". }
+by eauto.
+Qed.
+
+Lemma wp_connection_close E (c : val) cs n :
+  {{{ is_conn_state cs n }}}
+    Connection.close c (repr cs) @ E
+  {{{ RET #(); True }}}.
+Proof.
+iIntros "%Φ (conn & _) post".
+wp_lam; wp_pures.
+wp_free.
+by iApply "post".
+Qed.
+
+End Verif.
