store/server_proofs.v
@@ -4,11 +4,12 @@ From stdpp Require Import namespaces.
 From iris.algebra Require Import agree auth csum gset gmap excl frac.
 From iris.algebra Require Import max_prefix_list.
 From iris.heap_lang Require Import notation proofmode.
+From iris.heap_lang.lib Require Import ticket_lock.
 From cryptis Require Import lib version term cryptis primitives tactics.
-From cryptis Require Import role dh_auth.
-From cryptis.store Require Import impl shared alist db.
+From cryptis Require Import gmeta nown role dh_auth.
+From cryptis.store Require Import impl shared alist db connection_proofs.
 From cryptis.store.server_proofs
-  Require Import load store create.
+  Require Import load store create close.
 
 Set Implicit Arguments.
 Unset Strict Implicit.
@@ -16,12 +17,12 @@ Unset Printing Implicit Defensive.
 
 Section Verif.
 
-Context `{!cryptisGS Σ, !heapGS Σ, !sessionGS Σ}.
+Context `{!cryptisGS Σ, !heapGS Σ, !storeGS Σ, !tlockG Σ}.
 Notation iProp := (iProp Σ).
 
 Context `{!storeGS Σ}.
 
-Implicit Types (cs : cst) (ss : sst).
+Implicit Types (cs : conn_state).
 Implicit Types kI kR kS t : term.
 Implicit Types n : nat.
 Implicit Types γ : gname.
@@ -29,88 +30,208 @@ Implicit Types v : val.
 
 Variable N : namespace.
 
-Lemma wp_server_conn_handler_body E c ss :
+Lemma wp_server_conn_handler_body E c cs n ldb db :
   ↑cryptisN ⊆ E →
+  ↑nroot.@"db" ⊆ E →
   channel c -∗
   store_ctx N -∗
-  {{{ server ss }}}
-    Server.conn_handler_body N c (repr ss) @ E
-  {{{ v, RET v; server ss }}}.
+  {{{ is_conn_state cs n ∗
+      server_connected cs n db ∗
+      SAList.is_alist ldb (repr <$> db) }}}
+    Server.conn_handler_body N c (repr cs) ldb @ E
+  {{{ v, RET v; server_handler_post cs ldb v }}}.
 Proof.
-iIntros "% #chan_c #ctx !> %Φ state post". rewrite /Server.conn_handler_body.
-wp_pures. wp_bind (recv _). iApply wp_recv => //.
-iIntros "%m #p_m". wp_pures.
-wp_bind (Server.handle_store _ _ _ _).
-iApply (wp_server_handle_store with "chan_c ctx p_m state") => //.
-iIntros "!> %res state".
-case: res => [?|] /=; wp_pures; first by iApply "post".
-wp_bind (Server.handle_load _ _ _ _).
-iApply (wp_server_handle_load with "chan_c ctx p_m state") => //.
-iIntros "!> %res state".
-case: res => [?|] /=; wp_pures; first by iApply "post".
-wp_bind (Server.handle_create _ _ _ _).
-iApply (wp_server_handle_create with "chan_c ctx p_m state") => //.
-iIntros "!> %res state".
-case: res => [?|] /=; wp_pures; first by iApply "post".
+iIntros "% % #chan_c #ctx !> %Φ (conn & server & db) post".
+wp_lam. wp_pures.
+rewrite !Connection.subst_select /=.
+iApply (wp_wand with "[conn server db] post").
+iCombine "server db" as "I". iRevert "conn I".
+iApply wp_connection_select => //=; do !iSplitR => //.
+- by iApply wp_server_handle_store.
+- by iApply wp_server_handle_load.
+- by iApply wp_server_handle_create.
+- by iApply wp_server_handle_close.
+Qed.
+
+Lemma wp_server_conn_handler c cs n vdb db vlock γlock :
+  channel c -∗
+  is_lock γlock vlock (account_inv (si_init cs) (si_resp cs) vdb) -∗
+  store_ctx N -∗
+  {{{ is_conn_state cs n ∗
+      server_connected cs n db ∗
+      SAList.is_alist vdb (repr <$> db) ∗
+      locked γlock }}}
+    Server.conn_handler N c (repr cs) vdb vlock
+  {{{ RET #(); True }}}.
+Proof.
+iIntros "#chan_c #lock #ctx".
+iLöb as "IH" forall (n db).
+iIntros "!> %Φ (conn & server & db & locked) post".
+wp_rec. wp_pures. wp_bind (Server.conn_handler_body _ _ _ _).
+iApply (wp_server_conn_handler_body with "[# //] [# //] [$]") => //.
+iIntros "!> %v (%n' & %db' & [state|state])".
+- iDestruct "state" as "(-> & conn & server & db)".
+  wp_pures. by iApply ("IH" with "[$]").
+- iDestruct "state" as "(-> & conn & server & db)".
+  wp_pures. wp_bind (release _).
+  iApply (release_spec with "[lock locked server db]").
+  { iFrame "locked". iSplit => //.
+    iExists db'. by iFrame. }
+  iIntros "!> _". wp_pures.
+  by iApply (wp_connection_close with "conn").
+Qed.
+
+Lemma wp_server_find_client ss kI :
+  {{{ cryptis_ctx ∗ server ss }}}
+    Server.find_client (repr ss) (TKey Dec kI)
+  {{{ vdb γlock vlock, RET (vdb, vlock)%V;
+      server ss ∗
+      is_lock γlock vlock
+        (account_inv kI (ss_key ss) vdb) }}}.
+Proof.
+iIntros "%Φ [#ctx server] post".
+iDestruct "server"
+  as "(%γR & %accounts & %E & #p_vkR & accounts & #name & token &
+       %EP & #locks)".
+wp_lam; wp_pures.
+wp_bind (SAList.find _ _).
+iApply (SAList.wp_find with "accounts").
+iIntros "!> accounts"; rewrite lookup_fmap.
+case accounts_kI: (accounts !! TKey Dec kI) => [scs|]; wp_pures.
+- rewrite big_sepM_forall.
+  iPoseProof ("locks" $! (TKey Dec kI) scs with "[//]")
+    as "(%kI' & %e & #lock)".
+  case: e => <- {kI'}.
+  iModIntro.
+  iApply ("post" $! (scs_db scs) (scs_name scs) (scs_lock scs)).
+  iSplit => //.
+  iExists γR, accounts, E. iFrame.
+  rewrite big_sepM_forall. by eauto.
+- have ?: ↑dbSN kI ⊆ E.
+  { by apply: EP; rewrite elem_of_dom accounts_kI. }
+  rewrite (gmeta_token_difference _ (↑dbSN kI)) //.
+  iDestruct "token" as "[token_kI token]".
+  iAssert (db_not_signed_up kI (ss_key ss))
+    with "[token_kI]" as "not_signed_up".
+  { iExists γR. by iFrame. }
+  wp_bind (SAList.new #()).
+  iApply SAList.wp_empty => //.
+  iIntros "!> %vdb db". wp_pures.
+  wp_bind (newlock #()).
+  iApply (newlock_spec (account_inv kI (ss_key ss) vdb)
+           with "[not_signed_up db]").
+  { iExists ∅. iFrame.
+    iSplit; first by rewrite /public_db big_sepM_empty.
+    iRight. iLeft. by iFrame. }
+  iIntros "!> %vlock %γlock #lock".
+  wp_pures.
+  wp_bind (SAList.insert _ _ _).
+  iApply (SAList.wp_insert with "accounts").
+  iIntros "!> accounts". wp_pures.
+  pose scs := {| scs_db := vdb; scs_name := γlock; scs_lock := vlock |}.
+  rewrite -(fmap_insert _ _ _ scs).
+  iModIntro.
+  iApply ("post" $! vdb γlock vlock).
+  iSplit => //.
+  iExists γR, _, (E ∖ ↑dbSN kI).
+  iFrame.
+  do !iSplit => //.
+  + iPureIntro.
+    move=> kI'.
+    rewrite dom_insert elem_of_union elem_of_singleton.
+    case/Decidable.not_or => fresh1 fresh2.
+    have ?: kI' ≠ kI by congruence.
+    move/(_ _ fresh2) in EP.
+    solve_ndisj.
+  + rewrite big_sepM_insert => //.
+    iSplit => //.
+    iExists _. iSplit => //.
+Qed.
+
+Lemma wp_server_wait_init c cs vdb db γlock vlock :
+  cs_role cs = Resp →
+  {{{ cryptis_ctx ∗ channel c ∗ store_ctx N ∗
+      is_conn_state cs 0 ∗
+      server_connecting cs db ∗
+      conn_not_started cs Resp ∗
+      conn_not_ended cs Resp ∗
+      SAList.is_alist vdb (repr <$> db) ∗
+      is_lock γlock vlock (
+        account_inv (si_init cs) (si_resp cs) vdb) ∗
+      locked γlock }}}
+    Server.wait_init N c (repr cs) vdb vlock
+  {{{ RET #(); True }}} .
+Proof.
+iIntros "%e_rl %Φ
+  (#ctx & #chan_c & #ctx' & conn & server & not_started & not_ended &
+   db & #lock & locked) post".
+wp_lam; wp_pures.
+iPoseProof (store_ctx_init with "ctx'") as "?".
+iCombine "server not_started not_ended db locked post" as "I".
+iRevert "conn I".
+iApply wp_connection_recv => //.
+iIntros "!> %m conn
+  (server & not_started & not_ended & db & locked & post) #m_m #p_m".
+iMod (ack_init_predI with "server conn not_started not_ended p_m")
+  as "H" => //.
+wp_pures.
+iMod "H" as "(conn & server & #p_m')".
+wp_bind (tint _). iApply wp_tint.
+wp_bind (Connection.send _ _ _ _).
+iPoseProof (store_ctx_ack_init with "ctx'") as "?".
+iApply (wp_connection_send with "[//] [//] [] [//] conn") => //.
+{ by rewrite public_TInt. }
+iIntros "!> conn". wp_pures.
+wp_bind (Server.conn_handler _ _ _ _ _).
+iApply (wp_server_conn_handler with "[//] [//] [//] [$]").
+iIntros "!> _". wp_pures.
+iModIntro. iRight. iExists _. iSplit => //.
 by iApply "post".
 Qed.
 
-Lemma wp_server_conn_handler E c ss :
-  ↑cryptisN ⊆ E →
-  channel c -∗
-  store_ctx N -∗
-  {{{ server ss }}}
-    Server.conn_handler N c (repr ss) @ E
-  {{{ v, RET v; False }}}.
-Proof.
-iIntros "% #chan_c #ctx".
-iLöb as "IH". iIntros "!> %Φ state post". wp_rec.
-wp_pures. wp_bind (Server.conn_handler_body _ _ _).
-iApply (wp_server_conn_handler_body with "[# //] [# //] [$]") => //.
-iIntros "!> %n' state". wp_pures.
-by iApply ("IH" with "[$]").
-Qed.
-
-Lemma wp_server_listen E c kR dq ph T :
-  ↑cryptisN ⊆ E →
-  ↑N ⊆ E →
+Lemma wp_server_listen c ss dq ph T :
   {{{ cryptis_ctx ∗ channel c ∗ store_ctx N ∗
-      public (TKey Dec kR) ∗ ●H{dq|ph} T }}}
-    Server.listen N c (TKey Enc kR) (TKey Dec kR) @ E
-  {{{ RET #(); False }}}.
+      server ss ∗ ●H{dq|ph} T }}}
+    Server.listen N c (repr ss)
+  {{{ RET #(); server ss ∗ ●H{dq|ph} T }}}.
 Proof.
-iIntros "% %". iLöb as "IH".
-iIntros "%Φ (#? & #chan_c & #ctx & #p_ek & hon) post".
-wp_pures. wp_rec. wp_pures. wp_bind (responder _ _ _ _).
-iAssert (dh_auth_ctx (N.@"auth")) as "#?".
-  by iDestruct "ctx" as "(_ & _ & _ & _ & _ & _ & _ & ?)".
-iApply (wp_responder
-         with "[# //] [# //] [# //] [# //] [hon]") => //;
+iIntros "%Φ (#? & #chan_c & #ctx & server & hon) post".
+wp_lam; wp_pures.
+iPoseProof (store_ctx_dh_auth_ctx with "ctx") as "dh".
+wp_bind (Connection.listen _ _ _ _).
+iApply (wp_connection_listen
+         with "[# //] [# //] [# //] [#] [hon]") => //;
   try by solve_ndisj.
-iIntros "!> %res (hon & resP)". case: res => [[pkI kS]|]; wp_pures; last first.
-  iApply ("IH" with "[hon] [$]"). iFrame. by eauto.
-iDestruct "resP" as "(%kI & %γ & -> & #m_kI & #m_kS & #sessR & _ & #sec_key)".
-wp_bind (Fork _). iApply wp_fork; last first.
-  iModIntro. wp_pures. iApply ("IH" with "[-post] post"). iFrame.
-  by eauto.
-iClear "IH". iModIntro. rewrite /Server.wait_init. wp_pures.
-iAssert True%I as "I"; first by []. iRevert "I". iApply wp_sess_recv => //.
-iIntros "!> %t _ #p_t".
-wp_pures. wp_bind (AList.empty _).
-iApply AList.wp_empty => //. iIntros "!> %kvs %kvs0".
-wp_alloc ldb as "Hdb". wp_pures.
-wp_alloc ts as "Hts".
-iDestruct (initE with "[//] [//] [//] p_t") as "{p_t} p_t".
-set si := SessInfo _ _ _ _ _.
-pose (ss := {| sst_si := si;
-               sst_ts := ts;
-               sst_db := ldb; |}).
-iAssert (▷ server ss)%I with "[Hts Hdb]" as "state".
-{ iExists _, 0, kvs, ∅. iFrame.
-  rewrite big_sepM_empty. do 5!iSplitR => //. }
+{ by iDestruct "server" as "(% & % & % & ? & _)". }
+iIntros "!> %cs (hon & resP)". wp_pures.
+iDestruct "resP" as "(conn & %e_kR & <- & <- & %e_rl & token)".
+wp_bind (Server.find_client _ _).
+iApply (wp_server_find_client with "[$]").
+iIntros "!> %vdb %γlock %vlock [server #lock]".
+wp_pure _ credit:"c".
 wp_pures.
-iApply (wp_server_conn_handler _ ss with "[#] [#] [$]") => //.
-by iIntros "!> % []".
+wp_bind (acquire _).
+iApply acquire_spec => //.
+iIntros "!> (locked & %db & account & db)". rewrite -e_kR.
+iMod (server_connectingI with "[//] hon c account") as "[hon account]".
+wp_pures.
+iPoseProof (conn_state_session with "conn") as "#?".
+iAssert (|={⊤}=> conn_not_started cs Resp ∗ conn_not_ended cs Resp)%I
+  with "[token]" as ">[not_started not_ended]".
+{ rewrite (gmeta_token_difference _ (↑nroot.@"db".@"begin")); last by solve_ndisj.
+  iDestruct "token" as "[not_started token]".
+  iSplitR "token".
+  { iModIntro. iExists _. iFrame. by rewrite e_rl. }
+  rewrite (gmeta_token_difference _ (↑nroot.@"db".@"end")); last by solve_ndisj.
+  iDestruct "token" as "[not_ended token]".
+  iModIntro. iExists _. iFrame. by rewrite e_rl. }
+iApply (wp_fork with "[conn locked db account not_started not_ended]").
+{ iModIntro.
+  iApply (wp_server_wait_init
+           with "[conn locked db account not_started not_ended] []") => //.
+  iFrame. eauto. }
+iApply "post".
+by iFrame.
 Qed.
 
 End Verif.
