store/server_proofs/close.v
@@ -1,0 +1,66 @@
+From stdpp Require Import base gmap.
+From mathcomp Require Import ssreflect.
+From stdpp Require Import namespaces.
+From iris.algebra Require Import agree auth csum gset gmap excl frac.
+From iris.algebra Require Import max_prefix_list.
+From iris.heap_lang Require Import notation proofmode.
+From cryptis Require Import lib version term cryptis primitives tactics.
+From cryptis Require Import role dh_auth.
+From cryptis.store Require Import impl shared alist db connection_proofs.
+
+Set Implicit Arguments.
+Unset Strict Implicit.
+Unset Printing Implicit Defensive.
+
+Section Verif.
+
+Context `{!cryptisGS Σ, !heapGS Σ, !sessionGS Σ}.
+Notation iProp := (iProp Σ).
+
+Context `{!storeGS Σ}.
+
+Implicit Types (cs : conn_state).
+Implicit Types kI kR kS t : term.
+Implicit Types n : nat.
+Implicit Types γ : gname.
+Implicit Types v : val.
+
+Variable N : namespace.
+
+Ltac failure := iLeft; iFrame.
+
+Lemma wp_server_handle_close E c cs n ldb db :
+  ↑cryptisN ⊆ E →
+  ↑nroot.@"db" ⊆ E →
+  channel c -∗
+  store_ctx N -∗
+  handler_correct
+    (server_handler_inv cs n ldb db)
+    (server_handler_post cs ldb)
+    cs
+    (N.@"close", Server.handle_close N c (repr cs) ldb)
+    n E.
+Proof.
+iIntros "%sub %sub' #chan_c #ctx".
+iPoseProof (store_ctx_close with "ctx") as "?".
+iPoseProof (store_ctx_ack_close with "ctx") as "?".
+rewrite /handler_correct. wp_lam; wp_pures. iModIntro.
+iExists _. iSplit => //. iIntros "!> %m _ #p_m conn (server & db)".
+wp_pures. wp_bind (Connection.timestamp _).
+iApply (wp_connection_timestamp with "conn").
+iIntros "!> conn". wp_pures.
+wp_bind (to_int _). iApply wp_to_int.
+case: Spec.to_intP => [ {m} n' ->| _]; wp_pures; last by failure.
+case: bool_decide_reflect => [[<-] {n'}|?]; last by wp_pures; failure.
+iPoseProof (ack_close_predI with "conn server p_m") as "{p_m} >H" => //.
+wp_pures. iMod "H" as "(conn & server & #p_m)".
+wp_bind (tint _). iApply wp_tint.
+wp_bind (Connection.send _ _ _ _).
+iApply (wp_connection_send with "[//] [//] [] p_m conn") => //.
+- by rewrite public_TInt.
+iIntros "!> conn". wp_pures.
+iRight. iModIntro. iExists _. iSplit => //.
+iExists _, _. iRight. by iFrame.
+Qed.
+
+End Verif.
