store/server_proofs/load.v
@@ -4,9 +4,10 @@ From stdpp Require Import namespaces.
 From iris.algebra Require Import agree auth csum gset gmap excl frac.
 From iris.algebra Require Import max_prefix_list.
 From iris.heap_lang Require Import notation proofmode.
-From cryptis Require Import lib version term cryptis primitives tactics.
+From cryptis Require Import lib version term gmeta nown.
+From cryptis Require Import cryptis primitives tactics.
 From cryptis Require Import role dh_auth.
-From cryptis.store Require Import impl shared alist db.
+From cryptis.store Require Import impl shared alist db connection_proofs.
 
 Set Implicit Arguments.
 Unset Strict Implicit.
@@ -14,12 +15,12 @@ Unset Printing Implicit Defensive.
 
 Section Verif.
 
-Context `{!cryptisGS Σ, !heapGS Σ, !sessionGS Σ}.
+Context `{!cryptisGS Σ, !heapGS Σ, !storeGS Σ}.
 Notation iProp := (iProp Σ).
 
 Context `{!storeGS Σ}.
 
-Implicit Types (cs : cst) (ss : sst).
+Implicit Types (cs : conn_state).
 Implicit Types kI kR kS t : term.
 Implicit Types n : nat.
 Implicit Types γ : gname.
@@ -27,50 +28,43 @@ Implicit Types v : val.
 
 Variable N : namespace.
 
-Lemma wp_server_handle_load E c ss m :
+Ltac failure := iLeft; iFrame.
+
+Lemma wp_server_handle_load E c cs ldb db n :
   ↑cryptisN ⊆ E →
   channel c -∗
   store_ctx N -∗
-  public m -∗
-  {{{ server ss }}}
-    Server.handle_load N c (repr ss) m @ E
-  {{{ (v : option val), RET (repr v); server ss }}}.
+  handler_correct
+    (server_handler_inv cs n ldb db)
+    (server_handler_post cs ldb)
+    cs
+    (N.@"load", Server.handle_load N c (repr cs) ldb)
+    n E.
 Proof.
-iIntros "%sub #chan_c #ctx #p_m !> %Φ state post".
-rewrite /Server.handle_load. wp_pures.
-iDestruct "state" as "(%γ & %n & %kvs & %db & #sessR & #key & #minted_key & ts &
-                       db & %kvs_db & #pub_db & #view)".
-wp_load. wp_pures. wp_load. wp_pures.
-iAssert (server ss) with "[ts db view]" as "state".
-{ iExists γ, n, kvs, db. iFrame. eauto 8. }
-wp_tsdec m; wp_pures; last by iApply ("post" $! None).
-wp_list_of_term m; wp_pures; last by iApply ("post" $! None).
-wp_list_match => [timestamp t1 ->| _]; wp_pures; last by iApply ("post" $! None).
+iIntros "%sub #chan_c #ctx".
+iPoseProof (store_ctx_load with "ctx") as "?".
+iPoseProof (store_ctx_ack_load with "ctx") as "?".
+rewrite /handler_correct. wp_lam; wp_pures.
+iModIntro. iExists _. iSplit => //. iIntros "!> %m _ #p_m conn (server & db)".
+wp_pures.
+wp_bind (Connection.timestamp _).
+iApply (wp_connection_timestamp with "conn"). iIntros "!> conn".
+wp_pures.
+wp_list_of_term m; wp_pures; last by failure.
+wp_list_match => [timestamp t1 ->| _]; wp_pures; last by failure.
 wp_bind (to_int _). iApply wp_to_int.
-case: Spec.to_intP => [ {m} n' -> | _]; wp_pures; last by iApply ("post" $! None).
-case: bool_decide_reflect => [[<-]|?]; wp_pures; last by iApply ("post" $! None).
-wp_bind (AList.find _ _). iApply AList.wp_find => //.
-iIntros "!> _".
-rewrite lookup_fmap.
-case db_t1: (db !! t1) => [t2|]; wp_pures; last by iApply ("post" $! None).
+case: Spec.to_intP => [ {m} n' -> | _]; wp_pures; last by failure.
+case: bool_decide_reflect => [[<-]|?]; wp_pures; last by failure.
+wp_bind (SAList.find _ _). iApply (SAList.wp_find with "db") => //.
+iIntros "!> db". rewrite lookup_fmap.
+case db_t1: (db !! t1) => [t2|]; wp_pures; last by failure.
 wp_list. wp_bind (tint _). iApply wp_tint. wp_list. wp_term_of_list.
-wp_pures. wp_tsenc. wp_bind (send _ _).
-iApply (wp_send with "[//] [#]") => //; last by wp_pures;
-  iApply ("post" $! (Some #())).
-iDestruct "ctx" as "(_ & _ & _ & _ & ? & _)".
-iModIntro.
-rewrite big_sepM_delete //. iDestruct "pub_db" as "[[? ?] _]".
-iApply public_TEncIS => //.
-- rewrite minted_TKey.
-  iPoseProof (public_minted with "p_m") as "{p_m} p_m".
-  by rewrite minted_TEnc; iDestruct "p_m" as "[??]".
-- iModIntro. iExists n, t1, t2, ss, γ. iSplit => //.
-  do 3!iSplit => //.
-  iDestruct "view" as "[?|(%γ' & sessI & view)]"; first by iLeft.
-  iRight. iExists γ'. iSplit => //. iApply DB.load_server; eauto.
-- rewrite minted_of_list /= minted_TInt -[minted t1]public_minted.
-  rewrite -[minted t2]public_minted; eauto.
-- iIntros "!> _". by rewrite public_of_list /= public_TInt; eauto.
+wp_pures.
+iPoseProof (ack_load_predI db_t1 with "conn server") as "#[??]".
+wp_bind (Connection.send _ _ _ _).
+iApply (wp_connection_send with "[//] [//] [] [] conn") => //.
+iIntros "!> conn". wp_pures. iModIntro.
+iRight. iExists _. iSplit => //. iExists _, _. iLeft. by iFrame.
 Qed.
 
 End Verif.
