store/server_proofs/store.v
@@ -6,7 +6,7 @@ From iris.algebra Require Import max_prefix_list.
 From iris.heap_lang Require Import notation proofmode.
 From cryptis Require Import lib version term cryptis primitives tactics.
 From cryptis Require Import role dh_auth.
-From cryptis.store Require Import impl shared alist db.
+From cryptis.store Require Import impl shared alist db connection_proofs.
 
 Set Implicit Arguments.
 Unset Strict Implicit.
@@ -19,7 +19,7 @@ Notation iProp := (iProp Σ).
 
 Context `{!storeGS Σ}.
 
-Implicit Types (cs : cst) (ss : sst).
+Implicit Types (cs : conn_state).
 Implicit Types kI kR kS t : term.
 Implicit Types n : nat.
 Implicit Types γ : gname.
@@ -32,7 +32,7 @@ Lemma ack_storeI kS n :
   minted kS -∗
   public (TEnc kS (Spec.tag (N.@"ack_store") (TInt n))).
 Proof.
-iIntros "(_ & _ & #ctx & _) #s_kS".
+iIntros "(_ & _ & _ & #ctx & _) #s_kS".
 iApply public_TEncIS => //.
 - by rewrite minted_TKey.
 - iModIntro. by iExists n.
@@ -40,54 +40,49 @@ iApply public_TEncIS => //.
 - by rewrite public_TInt; eauto.
 Qed.
 
-Lemma wp_server_handle_store E c ss m :
+Ltac failure := iLeft; iFrame.
+
+Lemma wp_server_handle_store E c cs ldb db n :
   ↑cryptisN ⊆ E →
   channel c -∗
   store_ctx N -∗
-  public m -∗
-  {{{ server ss }}}
-    Server.handle_store N c (repr ss) m @ E
-  {{{ (v : option val), RET (repr v); server ss }}}.
+  handler_correct
+    (server_handler_inv cs n ldb db)
+    (server_handler_post cs ldb)
+    cs
+    (N.@"store", Server.handle_store N c (repr cs) ldb)
+    n E.
 Proof.
-iIntros "%sub #chan_c #ctx #p_m !> %Φ state post".
-rewrite /Server.handle_store. wp_pures.
-wp_tsdec m; wp_pures; last by iApply ("post" $! None).
-wp_list_of_term m; wp_pures; last by iApply ("post" $! None).
-wp_list_match => [n' t1 t2 ->|_]; wp_pures; last by iApply ("post" $! None).
+iIntros "%sub #chan_c #ctx".
+iPoseProof (store_ctx_store with "ctx") as "?".
+iPoseProof (store_ctx_ack_store with "ctx") as "?".
+rewrite /handler_correct /=. wp_lam; wp_pures.
+iModIntro. iExists _. iSplit => //.
+iIntros "!> %m _ #p_m conn (server & db)". wp_pures.
+wp_bind (Connection.timestamp _).
+iApply (wp_connection_timestamp with "conn") => //.
+iIntros "!> conn". wp_pures.
+wp_list_of_term m; wp_pures; last by failure.
+wp_list_match => [n' t1 t2 ->|_]; wp_pures; last by failure.
 wp_bind (to_int _). iApply wp_to_int.
-case: Spec.to_intP => [ {}n' -> | _]; wp_pures; last by iApply ("post" $! None).
-iDestruct "state" as "(%γ & %n & %kvs & %db & #sessR & #sec_key &
-                       #minted_key & ts & db & %kvs_db & #pub_db & view)".
-wp_load. wp_pures.
-case: bool_decide_reflect => [[<-]|ne]; wp_pures; last first.
-{ iModIntro. iApply ("post" $! None).
-  iExists γ, n, kvs, db. iFrame. by eauto. }
-wp_load. wp_pures.
-replace (n + 1)%Z with (S n : Z) by lia.
-wp_store. wp_load. wp_bind (AList.insert _ _ _).
-wp_pures. iApply AList.wp_insert; eauto. iIntros "!> %kvs' %kvs'_db'".
-iDestruct (store_predE with "[//] sessR sec_key [#] p_m")
-  as "(p_t1 & p_t2 & wf')".
-{ iDestruct "view" as "[#fail|(% & #? & ?)]".
-  - by iLeft.
-  - by iRight; eauto. }
-wp_store. wp_bind (tint _). iApply wp_tint.
-wp_tsenc.
-iApply wp_fupd.
-wp_bind (send _ _). iApply wp_send => //.
-{ iModIntro. iApply ack_storeI => //. }
-wp_pures. iApply ("post" $! (Some #())).
-iExists γ, (S n), kvs', (<[t1 := t2]>db). iFrame.
-rewrite -fmap_insert in kvs'_db'.
-do 4!iSplitR => //.
-iSplitR.
-{ iModIntro. iApply big_sepM_insert_2 => //. eauto. }
-iDestruct "wf'" as "[?|(%γ1 & sessI1 & update)]"; first by iLeft.
-iDestruct "view" as "[?|(%γ2 & #sessI2 & #view)]"; first by iLeft.
-iPoseProof (session_agree_name with "sessI1 sessI2") as "[?|(_ & ->)]" => //;
-  first by iLeft.
-iPoseProof (DB.update_server with "view update") as "view'".
-iIntros "!>". iRight. iExists _. iSplit => //.
+case: Spec.to_intP => [ {}n' -> | _]; wp_pures; last by failure.
+case: bool_decide_reflect => [[ {n'} <-]|ne]; wp_pures; last by failure.
+iPoseProof (store_predE with "conn server p_m") as "(conn & server)".
+wp_bind (Connection.tick _). iApply (wp_connection_tick with "conn").
+iIntros "!> conn". wp_pures.
+wp_bind (SAList.insert _ _ _).
+iApply (SAList.wp_insert with "db").
+iIntros "!> db". rewrite -fmap_insert.
+wp_pures.
+wp_bind (tint _). iApply wp_tint.
+wp_bind (Connection.send _ _ _ _).
+iApply (wp_connection_send _ c cs (S n)
+   with "[//] [//] [] [] conn [server db]") => //.
+- by rewrite public_TInt.
+- by iExists _.
+iIntros "!> conn". wp_pures.
+iModIntro. iRight. iExists _. iSplit => //.
+iExists _, _. iLeft. by iFrame.
 Qed.
 
 End Verif.
